Implement and verify uncross_shadow, which transforms an nnrc_impish statement into an equivalent one that is cross_shadow_free

coq/NNRCimpish/Lang/NNRCimpishCrossShadow.v
@@ -18,10 +18,12 @@
    a variable in another namespace.  This is not a problem for nnrc_impish, since 
    the namespaces are all distinct.  However, it poses a problem when compiling to
    a language like nnrc_imp that has a single namespace.
-*)
+ *)
 
 Require Import String.
 Require Import List.
+Require Import Permutation.
+Require Import ListSet.
 Require Import Arith.
 Require Import EquivDec.
 Require Import Morphisms.
@@ -34,82 +36,1356 @@ Require Import Decidable.
 Require Import Utils.
 Require Import CommonRuntime.
 Require Import NNRCimpish.
+Require Import NNRCimpishEval.
 Require Import NNRCimpishVars.
+Require Import NNRCimpishRename.
 
 Section NNRCimpishCrossShadow.
-
+  
   Context {fruntime:foreign_runtime}.
 
-  Context (h:brand_relation_t).
-
   Local Open Scope nnrc_impish.
-  Local Open Scope string.
 
-  Fixpoint nnrc_impish_stmt_cross_shadow_free_under
-           (s:nnrc_impish_stmt)
-           (σ ψc ψd:list var)
+  (** The definition of the cross shadow free predicate.  This definition is used by
+       the impish->imp translation.  If it holds, then collapsing namespaces is safe.
+   *)
+  Section def.
+    
+    Fixpoint nnrc_impish_stmt_cross_shadow_free_under
+             (s:nnrc_impish_stmt)
+             (σ ψc ψd:list var)
     : Prop
-    := match s with
-       | NNRCimpishSeq s₁ s₂ =>
-         nnrc_impish_stmt_cross_shadow_free_under s₁ σ ψc ψd
-         /\ nnrc_impish_stmt_cross_shadow_free_under s₂ σ ψc ψd
-       | NNRCimpishLet v e s₀ =>
-         disjoint (nnrc_impish_expr_free_vars e) ψc
-         /\ disjoint (nnrc_impish_expr_free_vars e) ψd
-        (* not the same: incl (nnrc_impish_expr_free_vars e) σ *)
-         /\ ~ In v ψc
-         /\ ~ In v ψd
-         /\ nnrc_impish_stmt_cross_shadow_free_under s₀ (v::σ) ψc ψd
-       | NNRCimpishLetMut v s₁ s₂ =>
-            ~ In v σ
-         /\ ~ In v ψc
-         /\ ~ In v ψd      
-         /\ nnrc_impish_stmt_cross_shadow_free_under s₁ σ ψc (v::ψd)
-         /\ nnrc_impish_stmt_cross_shadow_free_under s₂ (v::σ) ψc ψd
-       | NNRCimpishLetMutColl v s₁ s₂ =>
-            ~ In v σ
-         /\ ~ In v ψc
-         /\ ~ In v ψd      
-         /\ nnrc_impish_stmt_cross_shadow_free_under s₁ σ (v::ψc) ψd
-         /\ nnrc_impish_stmt_cross_shadow_free_under s₂ (v::σ) ψc ψd
-       | NNRCimpishAssign v e =>
-            disjoint (nnrc_impish_expr_free_vars e) ψc
-         /\ disjoint (nnrc_impish_expr_free_vars e) ψd
-         /\ ~ In v σ
-         /\ ~ In v ψc
-       (* not the same: In v ψd *)
-       | NNRCimpishPush v e =>
-         disjoint (nnrc_impish_expr_free_vars e) ψc
-         /\ disjoint (nnrc_impish_expr_free_vars e) ψd
-         /\ ~ In v σ
-         /\ ~ In v ψd
-       (* not the same: In v ψc *)
-       | NNRCimpishFor v e s₀ =>
-         disjoint (nnrc_impish_expr_free_vars e) ψc
-         /\ disjoint (nnrc_impish_expr_free_vars e) ψd
-        (* not the same: incl (nnrc_impish_expr_free_vars e) σ *)          
-         /\ ~ In v ψc
-         /\ ~ In v ψd
-         /\ nnrc_impish_stmt_cross_shadow_free_under s₀ (v::σ) ψc ψd
-       | NNRCimpishIf e s₁ s₂ =>
-         disjoint (nnrc_impish_expr_free_vars e) ψc
-         /\ disjoint (nnrc_impish_expr_free_vars e) ψd
-        (* not the same: incl (nnrc_impish_expr_free_vars e) σ *)
-         /\ nnrc_impish_stmt_cross_shadow_free_under s₁ σ ψc ψd
-         /\ nnrc_impish_stmt_cross_shadow_free_under s₂ σ ψc ψd
-       | NNRCimpishEither e x₁ s₁ x₂ s₂ =>
-         disjoint (nnrc_impish_expr_free_vars e) ψc
-         /\ disjoint (nnrc_impish_expr_free_vars e) ψd
-        (* not the same: incl (nnrc_impish_expr_free_vars e) σ *)
-         /\ ~ In x₁ ψc
-         /\ ~ In x₁ ψd
-         /\ ~ In x₂ ψc
-         /\ ~ In x₂ ψd
-         /\ nnrc_impish_stmt_cross_shadow_free_under s₁ (x₁::σ) ψc ψd
-         /\ nnrc_impish_stmt_cross_shadow_free_under s₂ (x₂::σ) ψc ψd
-       end.
+      := match s with
+         | NNRCimpishSeq s₁ s₂ =>
+           nnrc_impish_stmt_cross_shadow_free_under s₁ σ ψc ψd
+           /\ nnrc_impish_stmt_cross_shadow_free_under s₂ σ ψc ψd
+         | NNRCimpishLet v e s₀ =>
+           disjoint (nnrc_impish_expr_free_vars e) ψc
+           /\ disjoint (nnrc_impish_expr_free_vars e) ψd
+           (* not the same: incl (nnrc_impish_expr_free_vars e) σ *)
+           /\ ~ In v ψc
+           /\ ~ In v ψd
+           /\ nnrc_impish_stmt_cross_shadow_free_under s₀ (v::σ) ψc ψd
+         | NNRCimpishLetMut v s₁ s₂ =>
+           ~ In v σ
+           /\ ~ In v ψc
+           /\ ~ In v ψd      
+           /\ nnrc_impish_stmt_cross_shadow_free_under s₁ σ ψc (v::ψd)
+           /\ nnrc_impish_stmt_cross_shadow_free_under s₂ (v::σ) ψc ψd
+         | NNRCimpishLetMutColl v s₁ s₂ =>
+           ~ In v σ
+           /\ ~ In v ψc
+           /\ ~ In v ψd      
+           /\ nnrc_impish_stmt_cross_shadow_free_under s₁ σ (v::ψc) ψd
+           /\ nnrc_impish_stmt_cross_shadow_free_under s₂ (v::σ) ψc ψd
+         | NNRCimpishAssign v e =>
+           disjoint (nnrc_impish_expr_free_vars e) ψc
+           /\ disjoint (nnrc_impish_expr_free_vars e) ψd
+           /\ ~ In v σ
+           /\ ~ In v ψc
+         (* not the same: In v ψd *)
+         | NNRCimpishPush v e =>
+           disjoint (nnrc_impish_expr_free_vars e) ψc
+           /\ disjoint (nnrc_impish_expr_free_vars e) ψd
+           /\ ~ In v σ
+           /\ ~ In v ψd
+         (* not the same: In v ψc *)
+         | NNRCimpishFor v e s₀ =>
+           disjoint (nnrc_impish_expr_free_vars e) ψc
+           /\ disjoint (nnrc_impish_expr_free_vars e) ψd
+           (* not the same: incl (nnrc_impish_expr_free_vars e) σ *)          
+           /\ ~ In v ψc
+           /\ ~ In v ψd
+           /\ nnrc_impish_stmt_cross_shadow_free_under s₀ (v::σ) ψc ψd
+         | NNRCimpishIf e s₁ s₂ =>
+           disjoint (nnrc_impish_expr_free_vars e) ψc
+           /\ disjoint (nnrc_impish_expr_free_vars e) ψd
+           (* not the same: incl (nnrc_impish_expr_free_vars e) σ *)
+           /\ nnrc_impish_stmt_cross_shadow_free_under s₁ σ ψc ψd
+           /\ nnrc_impish_stmt_cross_shadow_free_under s₂ σ ψc ψd
+         | NNRCimpishEither e x₁ s₁ x₂ s₂ =>
+           disjoint (nnrc_impish_expr_free_vars e) ψc
+           /\ disjoint (nnrc_impish_expr_free_vars e) ψd
+           (* not the same: incl (nnrc_impish_expr_free_vars e) σ *)
+           /\ ~ In x₁ ψc
+           /\ ~ In x₁ ψd
+           /\ ~ In x₂ ψc
+           /\ ~ In x₂ ψd
+           /\ nnrc_impish_stmt_cross_shadow_free_under s₁ (x₁::σ) ψc ψd
+           /\ nnrc_impish_stmt_cross_shadow_free_under s₂ (x₂::σ) ψc ψd
+         end.
 
-  Definition nnrc_impish_cross_shadow_free (s:nnrc_impish)
-    := nnrc_impish_stmt_cross_shadow_free_under (fst s) nil nil (snd s::nil).
+    Definition nnrc_impish_cross_shadow_free (s:nnrc_impish)
+      := nnrc_impish_stmt_cross_shadow_free_under (fst s) nil nil (snd s::nil).
+
+  End def.
+
+  (** If the cross shadow predicate holds, then the environments in question 
+      must obey certain disjointness conditions *)
+  Section cross_shadow_free_disjointness.
+
+    Lemma nnrc_impish_stmt_cross_shadow_free_under_free_mcenv_env
+          (s:nnrc_impish_stmt) (σ ψc ψd:list var) :
+      nnrc_impish_stmt_cross_shadow_free_under s σ ψc ψd ->
+      disjoint (nnrc_impish_stmt_free_mcenv_vars s) σ.
+    Proof.
+      unfold disjoint.
+      revert σ ψc ψd
+      ; nnrc_impish_stmt_cases (induction s) Case
+      ; simpl; intros σ ψc ψd sf x inn.
+      - Case "NNRCimpishSeq"%string.
+        rewrite in_app_iff in inn.
+        intuition eauto.
+      - Case "NNRCimpishLet"%string.
+        intuition.
+        eapply IHs; eauto; simpl; eauto.
+      - Case "NNRCimpishLetMut"%string.
+        rewrite in_app_iff in inn.
+        intuition eauto.
+        eapply IHs2; eauto; simpl; eauto.
+      - Case "NNRCimpishLetMutColl"%string.
+        rewrite in_app_iff in inn.
+        intuition eauto.
+        + apply remove_inv in H4.
+          eapply IHs1; eauto; tauto.
+        + eapply IHs2; eauto; simpl; eauto.
+      - Case "NNRCimpishAssign"%string.
+        contradiction.
+      - Case "NNRCimpishPush"%string.
+        intuition congruence.
+      - Case "NNRCimpishFor"%string.
+        intuition.
+        eapply IHs; eauto; simpl; eauto.
+      - Case "NNRCimpishIf"%string.
+        repeat rewrite in_app_iff in inn.
+        intuition eauto. 
+      - Case "NNRCimpishEither"%string.
+        repeat rewrite in_app_iff in inn.
+        intuition.
+        + eapply IHs1; eauto; simpl; eauto.
+        + eapply IHs2; eauto; simpl; eauto.
+    Qed.
+
+    Lemma nnrc_impish_stmt_cross_shadow_free_under_free_mdenv_env
+          (s:nnrc_impish_stmt) (σ ψc ψd:list var) :
+      nnrc_impish_stmt_cross_shadow_free_under s σ ψc ψd ->
+      disjoint (nnrc_impish_stmt_free_mdenv_vars s) σ.
+    Proof.
+      unfold disjoint.
+      revert σ ψc ψd
+      ; nnrc_impish_stmt_cases (induction s) Case
+      ; simpl; intros σ ψc ψd sf x inn.
+      - Case "NNRCimpishSeq"%string.
+        rewrite in_app_iff in inn.
+        intuition eauto.
+      - Case "NNRCimpishLet"%string.
+        intuition.
+        eapply IHs; eauto; simpl; eauto.
+      - Case "NNRCimpishLetMut"%string.
+        rewrite in_app_iff in inn.
+        intuition eauto.
+        + apply remove_inv in H4.
+          eapply IHs1; eauto; tauto.
+        + eapply IHs2; eauto; simpl; eauto.
+      - Case "NNRCimpishLetMutColl"%string.
+        rewrite in_app_iff in inn.
+        intuition eauto.
+        eapply IHs2; eauto; simpl; eauto.
+      - Case "NNRCimpishAssign"%string.
+        intuition congruence.
+      - Case "NNRCimpishPush"%string.
+        contradiction.
+      - Case "NNRCimpishFor"%string.
+        intuition.
+        eapply IHs; eauto; simpl; eauto.
+      - Case "NNRCimpishIf"%string.
+        repeat rewrite in_app_iff in inn.
+        intuition eauto. 
+      - Case "NNRCimpishEither"%string.
+        repeat rewrite in_app_iff in inn.
+        intuition.
+        + eapply IHs1; eauto; simpl; eauto.
+        + eapply IHs2; eauto; simpl; eauto.
+    Qed.
+
+    Lemma nnrc_impish_stmt_cross_shadow_free_under_free_env_mcenv
+          (s:nnrc_impish_stmt) (σ ψc ψd:list var) :
+      nnrc_impish_stmt_cross_shadow_free_under s σ ψc ψd ->
+      disjoint (nnrc_impish_stmt_free_env_vars s) ψc.
+    Proof.
+      unfold disjoint.
+      revert σ ψc ψd
+      ; nnrc_impish_stmt_cases (induction s) Case
+      ; simpl; intros σ ψc ψd sf x inn.
+      - Case "NNRCimpishSeq"%string.
+        rewrite in_app_iff in inn.
+        intuition eauto.
+      - Case "NNRCimpishLet"%string.
+        rewrite in_app_iff in inn.
+        intuition eauto.
+        apply remove_inv in H4.
+        eapply IHs; eauto; simpl; tauto.
+      - Case "NNRCimpishLetMut"%string.
+        rewrite in_app_iff in inn.
+        intuition eauto.
+        apply remove_inv in H4.
+        eapply IHs2; eauto; simpl; tauto.
+      - Case "NNRCimpishLetMutColl"%string.
+        rewrite in_app_iff in inn.
+        intuition eauto.
+        + eapply IHs1; eauto; simpl; eauto. 
+        + apply remove_inv in H4.
+          eapply IHs2; eauto; tauto.
+      - Case "NNRCimpishAssign"%string.
+        intuition eauto.
+      - Case "NNRCimpishPush"%string.
+        intuition eauto.
+      - Case "NNRCimpishFor"%string.
+        rewrite in_app_iff in inn.
+        intuition eauto.
+        apply remove_inv in H4.
+        eapply IHs; eauto; simpl; tauto.
+      - Case "NNRCimpishIf"%string.
+        repeat rewrite in_app_iff in inn.
+        intuition eauto. 
+      - Case "NNRCimpishEither"%string.
+        repeat rewrite in_app_iff in inn.
+        intuition.
+        + eapply H0; eauto.
+        + apply remove_inv in H9.
+          eapply IHs1; eauto; tauto.
+        + apply remove_inv in H9.
+          eapply IHs2; eauto; tauto.
+    Qed.
+
+    Lemma nnrc_impish_stmt_cross_shadow_free_under_free_mdenv_mcenv
+          (s:nnrc_impish_stmt) (σ ψc ψd:list var) :
+      nnrc_impish_stmt_cross_shadow_free_under s σ ψc ψd ->
+      disjoint (nnrc_impish_stmt_free_mdenv_vars s) ψc.
+    Proof.
+      unfold disjoint.
+      revert σ ψc ψd
+      ; nnrc_impish_stmt_cases (induction s) Case
+      ; simpl; intros σ ψc ψd sf x inn.
+      - Case "NNRCimpishSeq"%string.
+        rewrite in_app_iff in inn.
+        intuition eauto.
+      - Case "NNRCimpishLet"%string.
+        intuition.
+        eapply IHs; eauto; simpl; eauto.
+      - Case "NNRCimpishLetMut"%string.
+        rewrite in_app_iff in inn.
+        intuition eauto.
+        apply remove_inv in H4.
+        eapply IHs1; eauto; tauto.
+      - Case "NNRCimpishLetMutColl"%string.
+        rewrite in_app_iff in inn.
+        intuition eauto.
+        eapply IHs1; eauto; simpl; eauto.
+      - Case "NNRCimpishAssign"%string.
+        intuition congruence.
+      - Case "NNRCimpishPush"%string.
+        contradiction.
+      - Case "NNRCimpishFor"%string.
+        intuition.
+        eapply IHs; eauto; simpl; eauto.
+      - Case "NNRCimpishIf"%string.
+        repeat rewrite in_app_iff in inn.
+        intuition eauto. 
+      - Case "NNRCimpishEither"%string.
+        repeat rewrite in_app_iff in inn.
+        intuition.
+        + eapply IHs1; eauto; simpl; eauto.
+        + eapply IHs2; eauto; simpl; eauto.
+    Qed.
+
+    Lemma nnrc_impish_stmt_cross_shadow_free_under_free_env_mdenv
+          (s:nnrc_impish_stmt) (σ ψc ψd:list var) :
+      nnrc_impish_stmt_cross_shadow_free_under s σ ψc ψd ->
+      disjoint (nnrc_impish_stmt_free_env_vars s) ψd.
+    Proof.
+      unfold disjoint.
+      revert σ ψc ψd
+      ; nnrc_impish_stmt_cases (induction s) Case
+      ; simpl; intros σ ψc ψd sf x inn.
+      - Case "NNRCimpishSeq"%string.
+        rewrite in_app_iff in inn.
+        intuition eauto.
+      - Case "NNRCimpishLet"%string.
+        rewrite in_app_iff in inn.
+        intuition eauto.
+        apply remove_inv in H4.
+        eapply IHs; eauto; simpl; tauto.
+      - Case "NNRCimpishLetMut"%string.
+        rewrite in_app_iff in inn.
+        intuition eauto.
+        + eapply IHs1; eauto; simpl; tauto.
+        + apply remove_inv in H4.
+          eapply IHs2; eauto; simpl; tauto.
+      - Case "NNRCimpishLetMutColl"%string.
+        rewrite in_app_iff in inn.
+        intuition eauto.
+        apply remove_inv in H4.
+        eapply IHs2; eauto; tauto.
+      - Case "NNRCimpishAssign"%string.
+        intuition eauto.
+      - Case "NNRCimpishPush"%string.
+        intuition eauto.
+      - Case "NNRCimpishFor"%string.
+        rewrite in_app_iff in inn.
+        intuition eauto.
+        apply remove_inv in H4.
+        eapply IHs; eauto; simpl; tauto.
+      - Case "NNRCimpishIf"%string.
+        repeat rewrite in_app_iff in inn.
+        intuition eauto. 
+      - Case "NNRCimpishEither"%string.
+        repeat rewrite in_app_iff in inn.
+        intuition.
+        + eapply H2; eauto.
+        + apply remove_inv in H9.
+          eapply IHs1; eauto; tauto.
+        + apply remove_inv in H9.
+          eapply IHs2; eauto; tauto.
+    Qed.
+
+    Lemma nnrc_impish_stmt_cross_shadow_free_under_free_mcenv_mdenv
+          (s:nnrc_impish_stmt) (σ ψc ψd:list var) :
+      nnrc_impish_stmt_cross_shadow_free_under s σ ψc ψd ->
+      disjoint (nnrc_impish_stmt_free_mcenv_vars s) ψd.
+    Proof.
+      unfold disjoint.
+      revert σ ψc ψd
+      ; nnrc_impish_stmt_cases (induction s) Case
+      ; simpl; intros σ ψc ψd sf x inn.
+      - Case "NNRCimpishSeq"%string.
+        rewrite in_app_iff in inn.
+        intuition eauto.
+      - Case "NNRCimpishLet"%string.
+        intuition.
+        eapply IHs; eauto; simpl; eauto.
+      - Case "NNRCimpishLetMut"%string.
+        rewrite in_app_iff in inn.
+        intuition eauto.
+        eapply IHs1; eauto; simpl; tauto.
+      - Case "NNRCimpishLetMutColl"%string.
+        rewrite in_app_iff in inn.
+        intuition eauto.
+        apply remove_inv in H4.
+        eapply IHs1; eauto; tauto.
+      - Case "NNRCimpishAssign"%string.
+        contradiction.
+      - Case "NNRCimpishPush"%string.
+        intuition congruence.
+      - Case "NNRCimpishFor"%string.
+        intuition.
+        eapply IHs; eauto; simpl; eauto.
+      - Case "NNRCimpishIf"%string.
+        repeat rewrite in_app_iff in inn.
+        intuition eauto. 
+      - Case "NNRCimpishEither"%string.
+        repeat rewrite in_app_iff in inn.
+        intuition.
+        + eapply IHs1; eauto; simpl; eauto.
+        + eapply IHs2; eauto; simpl; eauto.
+    Qed.
+    
+    Lemma nnrc_impish_stmt_cross_shadow_free_under_free_env_cons
+          {s:nnrc_impish_stmt} {σ ψc ψd:list var} {v} :
+      nnrc_impish_stmt_cross_shadow_free_under s (v::σ) ψc ψd ->
+      ~ In v (nnrc_impish_stmt_free_mcenv_vars s) /\ ~ In v (nnrc_impish_stmt_free_mdenv_vars s).
+    Proof.
+      intros sf; split; intros inn.
+      - eapply nnrc_impish_stmt_cross_shadow_free_under_free_mcenv_env; eauto
+        ;  simpl; eauto.
+      - eapply nnrc_impish_stmt_cross_shadow_free_under_free_mdenv_env; eauto
+        ;  simpl; eauto.
+    Qed.
+
+    Lemma nnrc_impish_stmt_cross_shadow_free_under_free_mcenv_cons
+          {s:nnrc_impish_stmt} {σ ψc ψd:list var} {v} :
+      nnrc_impish_stmt_cross_shadow_free_under s σ (v::ψc) ψd ->
+      ~ In v (nnrc_impish_stmt_free_env_vars s) /\ ~ In v (nnrc_impish_stmt_free_mdenv_vars s).
+    Proof.
+      intros sf; split; intros inn.
+      - eapply nnrc_impish_stmt_cross_shadow_free_under_free_env_mcenv; eauto
+        ;  simpl; eauto.
+      - eapply nnrc_impish_stmt_cross_shadow_free_under_free_mdenv_mcenv; eauto
+        ;  simpl; eauto.
+    Qed.
+
+    Lemma nnrc_impish_stmt_cross_shadow_free_under_free_mdenv_cons
+          {s:nnrc_impish_stmt} {σ ψc ψd:list var} {v} :
+      nnrc_impish_stmt_cross_shadow_free_under s σ ψc (v::ψd) ->
+      ~ In v (nnrc_impish_stmt_free_env_vars s) /\ ~ In v (nnrc_impish_stmt_free_mcenv_vars s).
+    Proof.
+      intros sf; split; intros inn.
+      - eapply nnrc_impish_stmt_cross_shadow_free_under_free_env_mdenv; eauto
+        ;  simpl; eauto.
+      - eapply nnrc_impish_stmt_cross_shadow_free_under_free_mcenv_mdenv; eauto
+        ;  simpl; eauto.
+    Qed.
+
+    Lemma nnrc_impish_stmt_cross_shadow_free_under_free_cons
+          (s:nnrc_impish_stmt) (σ ψc ψd:list var) v :
+      (nnrc_impish_stmt_cross_shadow_free_under s (v::σ) ψc ψd ->
+       ~ In v (nnrc_impish_stmt_free_mcenv_vars s) /\ ~ In v (nnrc_impish_stmt_free_mdenv_vars s))
+      /\ (nnrc_impish_stmt_cross_shadow_free_under s σ (v::ψc) ψd ->
+          ~ In v (nnrc_impish_stmt_free_env_vars s) /\ ~ In v (nnrc_impish_stmt_free_mdenv_vars s))
+      /\ (nnrc_impish_stmt_cross_shadow_free_under s σ ψc (v::ψd) ->
+          ~ In v (nnrc_impish_stmt_free_env_vars s) /\ ~ In v (nnrc_impish_stmt_free_mcenv_vars s))
+
+    .
+    Proof.
+      split; [ | split ].
+      -  apply nnrc_impish_stmt_cross_shadow_free_under_free_env_cons.
+      -  apply nnrc_impish_stmt_cross_shadow_free_under_free_mcenv_cons.
+      -  apply nnrc_impish_stmt_cross_shadow_free_under_free_mdenv_cons.
+    Qed.
+
+  End cross_shadow_free_disjointness.
+
+  (** The cross shadow predicate is preserved by equivalence an inclusion of the variable lists *)
+  Section cross_shadow_free_equivs.
+    
+    Global Instance nnrc_impish_stmt_cross_shadow_free_under_equivs :
+      Proper (eq ==> equivlist ==> equivlist ==> equivlist ==> iff) nnrc_impish_stmt_cross_shadow_free_under.
+    Proof.
+      cut (Proper (eq ==> equivlist ==> equivlist ==> equivlist ==> Basics.impl) nnrc_impish_stmt_cross_shadow_free_under).
+      {
+        unfold Proper, respectful, equivlist; unfold Basics.impl; split; [eauto | ].
+        symmetry in H1, H2, H3; eauto.
+      }
+      Ltac re_equivs_tac
+        := match goal with
+           | [H1: equivlist ?x ?y, H2: In ?v ?x, H3: In ?v ?y -> False |- _ ] =>
+             rewrite H1 in H2; contradiction
+           | [H1: equivlist ?y ?x, H2: In ?v ?x, H3: In ?v ?y -> False |- _ ] =>
+             rewrite <- H1 in H2; contradiction
+           | [ H1: equivlist ?x ?y, H2: disjoint _ ?x |- _ ] => rewrite H1 in H2
+           | [ H1: equivlist ?x ?y |- disjoint _ ?x] => rewrite H1
+           | [ |- equivlist (?x :: _ ) (?x :: _ ) ] => apply equivlist_cons_proper; [reflexivity | ]
+           end.
+
+      unfold Proper, respectful, Basics.impl; intros ? s ?; subst.
+      nnrc_impish_stmt_cases (induction s) Case
+      ; simpl; intros.
+      -  Case "NNRCimpishSeq"%string.
+         intuition eauto.
+      -  Case "NNRCimpishLet"%string.
+         intuition; repeat re_equivs_tac; eauto 2.
+         + eapply (IHs (v::x)); eauto.
+           re_equivs_tac; trivial.
+      - Case "NNRCimpishLetMut"%string.
+        intuition; repeat re_equivs_tac; eauto 2.
+        + eapply IHs1; (try (eapply equivlist_cons; trivial; eapply H1)); eauto.
+        + eapply IHs2; eauto. 
+          re_equivs_tac; trivial.
+      - Case "NNRCimpishLetMutColl"%string.
+        intuition; repeat re_equivs_tac; eauto 2.
+        + eapply IHs1; (try (eapply equivlist_cons; trivial; eapply H0)); eauto.
+        + eapply IHs2; eauto. 
+          re_equivs_tac; trivial.
+      - Case "NNRCimpishAssign"%string.
+        intuition; repeat re_equivs_tac; eauto 2.
+      - Case "NNRCimpishPush"%string.
+        intuition; repeat re_equivs_tac; eauto 2.
+      - Case "NNRCimpishFor"%string.
+        intuition; repeat re_equivs_tac; eauto 2.
+        + eapply (IHs (v::x)); eauto.
+          re_equivs_tac; trivial.
+      - Case "NNRCimpishIf"%string.
+        intuition; repeat re_equivs_tac; eauto 2.
+      - Case "NNRCimpishEither"%string.
+        intuition; repeat re_equivs_tac; eauto 2.
+        + eapply IHs1; eauto; re_equivs_tac; trivial.
+        + eapply IHs2; eauto; re_equivs_tac; trivial.
+    Qed.
+
+    Global Instance nnrc_impish_stmt_cross_shadow_free_under_incls :
+      Proper (eq ==> (@incl string) --> (@incl string) --> (@incl string) --> Basics.impl) nnrc_impish_stmt_cross_shadow_free_under.
+    Proof.
+      Ltac re_incl_tac
+        := match goal with
+           | [H1: incl ?x ?y, H2: In ?v ?x, H3: In ?v ?y -> False |- _ ] =>
+             rewrite H1 in H2; contradiction
+           | [H1: incl ?y ?x, H2: In ?v ?x, H3: In ?v ?y -> False |- _ ] =>
+             rewrite <- H1 in H2; contradiction
+           | [ H1: incl ?x ?y, H2: disjoint _ ?x |- _ ] => rewrite H1 in H2
+           | [ H1: incl ?x ?y |- disjoint _ ?x] => rewrite H1
+           | [ |- incl (?x :: _ ) (?x :: _ ) ] => apply incl_cons_proper; [reflexivity | ]
+           end.
+
+      Ltac re_incl_tact := intuition; try solve [repeat re_incl_tac; intuition].
+
+
+      unfold Proper, respectful, Basics.impl, Basics.flip; intros ? s ?; subst.
+      nnrc_impish_stmt_cases (induction s) Case
+      ; simpl; intros.
+      -  Case "NNRCimpishSeq"%string.
+         intuition eauto.
+      -  Case "NNRCimpishLet"%string.
+         re_incl_tact.
+         + eapply (IHs (v::x)); eauto.
+           re_incl_tact.
+      - Case "NNRCimpishLetMut"%string.
+        re_incl_tact.
+        + eapply IHs1; (try (eapply incl_cons_proper; trivial; eapply H1)); eauto.
+        + eapply IHs2; eauto. 
+          re_incl_tact.
+      - Case "NNRCimpishLetMutColl"%string.
+        re_incl_tact.
+        + eapply IHs1; (try (eapply incl_cons_proper; trivial; eapply H0)); eauto.
+        + eapply IHs2; eauto. 
+          re_incl_tact.
+      - Case "NNRCimpishAssign"%string.
+        re_incl_tact.
+      - Case "NNRCimpishPush"%string.
+        re_incl_tact.
+      - Case "NNRCimpishFor"%string.
+        re_incl_tact.
+        + eapply (IHs (v::x)); eauto.
+          re_incl_tact.
+      - Case "NNRCimpishIf"%string.
+        re_incl_tact; eauto.
+      - Case "NNRCimpishEither"%string.
+        re_incl_tact.
+        + eapply IHs1; eauto; re_incl_tact.
+        + eapply IHs2; eauto; re_incl_tact.
+    Qed.
+
+  End cross_shadow_free_equivs.
+
+  (** The cross shadow under predicate is "top down".  This version is more bottom up.
+        The former is easier for the translation to work with, the latter for the uncross_shadow transformation introduced later.
+        The latter implies the former for suitably disjoint variable lists.
+   *)
+
+  Section cross_shadow_free_alt.
+
+    Fixpoint nnrc_impish_stmt_cross_shadow_free_alt
+             (s:nnrc_impish_stmt)
+    : Prop
+      := match s with
+         | NNRCimpishSeq s₁ s₂ =>
+           nnrc_impish_stmt_cross_shadow_free_alt s₁
+           /\ nnrc_impish_stmt_cross_shadow_free_alt s₂
+         | NNRCimpishLet v e s₀ =>
+           ~ In v (nnrc_impish_stmt_free_mcenv_vars s₀)
+           /\ ~ In v (nnrc_impish_stmt_bound_mcenv_vars s₀)
+           /\ ~ In v (nnrc_impish_stmt_free_mdenv_vars s₀)
+           /\ ~ In v (nnrc_impish_stmt_bound_mdenv_vars s₀)
+           /\ nnrc_impish_stmt_cross_shadow_free_alt s₀
+         | NNRCimpishLetMut v s₁ s₂ =>
+           ~ In v (nnrc_impish_stmt_free_env_vars s₁)
+           /\ ~ In v (nnrc_impish_stmt_bound_env_vars s₁)
+           /\ ~ In v (nnrc_impish_stmt_free_mcenv_vars s₁)
+           /\ ~ In v (nnrc_impish_stmt_bound_mcenv_vars s₁)
+           /\ ~ In v (nnrc_impish_stmt_free_mcenv_vars s₂)
+           /\ ~ In v (nnrc_impish_stmt_bound_mcenv_vars s₂)
+           /\ ~ In v (nnrc_impish_stmt_bound_mdenv_vars s₂)
+           /\ ~ In v (nnrc_impish_stmt_free_mdenv_vars s₂)
+           /\ nnrc_impish_stmt_cross_shadow_free_alt s₁
+           /\ nnrc_impish_stmt_cross_shadow_free_alt s₂
+         | NNRCimpishLetMutColl v s₁ s₂ =>
+           ~ In v (nnrc_impish_stmt_free_env_vars s₁)
+           /\ ~ In v (nnrc_impish_stmt_bound_env_vars s₁)
+           /\ ~ In v (nnrc_impish_stmt_free_mdenv_vars s₁)
+           /\ ~ In v (nnrc_impish_stmt_bound_mdenv_vars s₁)
+           /\ ~ In v (nnrc_impish_stmt_free_mcenv_vars s₂)
+           /\ ~ In v (nnrc_impish_stmt_bound_mcenv_vars s₂)
+           /\ ~ In v (nnrc_impish_stmt_bound_mdenv_vars s₂)
+           /\ ~ In v (nnrc_impish_stmt_free_mdenv_vars s₂)
+           /\ nnrc_impish_stmt_cross_shadow_free_alt s₁
+           /\ nnrc_impish_stmt_cross_shadow_free_alt s₂ 
+         | NNRCimpishAssign v e => True
+         | NNRCimpishPush v e => True
+         | NNRCimpishFor v e s₀ =>
+           ~ In v (nnrc_impish_stmt_free_mcenv_vars s₀)
+           /\ ~ In v (nnrc_impish_stmt_bound_mcenv_vars s₀)
+           /\ ~ In v (nnrc_impish_stmt_free_mdenv_vars s₀)
+           /\ ~ In v (nnrc_impish_stmt_bound_mdenv_vars s₀)
+           /\ nnrc_impish_stmt_cross_shadow_free_alt s₀
+         | NNRCimpishIf e s₁ s₂ =>
+           nnrc_impish_stmt_cross_shadow_free_alt s₁
+           /\ nnrc_impish_stmt_cross_shadow_free_alt s₂
+         | NNRCimpishEither e x₁ s₁ x₂ s₂ =>
+           ~ In x₁ (nnrc_impish_stmt_free_mcenv_vars s₁)
+           /\ ~ In x₁ (nnrc_impish_stmt_bound_mcenv_vars s₁)
+           /\ ~ In x₁ (nnrc_impish_stmt_free_mdenv_vars s₁)
+           /\ ~ In x₁ (nnrc_impish_stmt_bound_mdenv_vars s₁)
+           /\ ~ In x₂ (nnrc_impish_stmt_free_mcenv_vars s₂)
+           /\ ~ In x₂ (nnrc_impish_stmt_bound_mcenv_vars s₂)
+           /\ ~ In x₂ (nnrc_impish_stmt_free_mdenv_vars s₂)
+           /\ ~ In x₂ (nnrc_impish_stmt_bound_mdenv_vars s₂)
+           /\ nnrc_impish_stmt_cross_shadow_free_alt s₁ 
+           /\ nnrc_impish_stmt_cross_shadow_free_alt s₂ 
+         end.
+
+    Ltac disj_tac :=
+      repeat
+        (match goal with
+         | [ H : disjoint (_ ++ _) _ |- _ ] => apply disjoint_app_l in H; destruct H
+         | [ H : disjoint (_ :: _) _ |- _ ] => apply disjoint_cons_inv1 in H; destruct H
+         | [ H : disjoint _ (_ :: _) |- _ ] => apply disjoint_cons_inv2 in H; destruct H
+         | [H1:disjoint (remove _ ?v ?l1) ?l2,
+               H2:In ?v ?l1 -> False |- _ ] => rewrite nin_remove in H1 by apply H2
+         | [H1:disjoint (remove _ ?v ?l1) ?l2,
+               H2:~ In ?v ?l1 |- _ ] => rewrite nin_remove in H1 by apply H2
+         | [H1:disjoint (remove _ ?v ?l1) ?l2,
+               H2:In ?v ?l2 -> False |- _ ] => rewrite disjoint_remove_swap in H1; rewrite nin_remove in H1 by apply H2
+         | [H1:disjoint (remove _ ?v ?l1) ?l2,
+               H2:~ In ?v ?l2 |- _ ] => rewrite disjoint_remove_swap in H1; rewrite nin_remove in H1 by apply H2
+         | [H : In _ (replace_all _ _ _ ) |- _ ] => apply in_replace_all in H; try solve [destruct H as [?|[??]]; subst; eauto]
+         | [H: ~ In _ (remove _ _ _) |- _ ] => try rewrite <- remove_in_neq in H by congruence
+         | [H: In _ (remove _ _ _) -> False |- _ ] => try rewrite <- remove_in_neq in H by congruence
+         | [ |- disjoint (_ :: _) _ ] => apply disjoint_cons1
+         | [ |- disjoint _ (_ :: _) ] => apply disjoint_cons2
+         | [ |- disjoint _ (replace_all _ _ _ )] => try solve [apply disjoint_replace_all; intuition]
+                                                        
+         end; repeat rewrite in_app_iff in *
+        ).
+
+    Theorem  nnrc_impish_stmt_cross_shadow_free_under_alt
+             (s:nnrc_impish_stmt) :
+      nnrc_impish_stmt_cross_shadow_free_alt s ->
+      forall (σ ψc ψd:list var),
+        disjoint (nnrc_impish_stmt_free_mcenv_vars s) σ ->
+        disjoint (nnrc_impish_stmt_bound_mcenv_vars s) σ ->
+        disjoint (nnrc_impish_stmt_free_mdenv_vars s) σ ->
+        disjoint (nnrc_impish_stmt_bound_mdenv_vars s) σ ->
+        disjoint (nnrc_impish_stmt_free_env_vars s) ψc ->
+        disjoint (nnrc_impish_stmt_bound_env_vars s) ψc ->
+        disjoint (nnrc_impish_stmt_free_mdenv_vars s) ψc ->
+        disjoint (nnrc_impish_stmt_bound_mdenv_vars s) ψc ->
+        disjoint (nnrc_impish_stmt_free_env_vars s) ψd ->
+        disjoint (nnrc_impish_stmt_bound_env_vars s) ψd ->
+        disjoint (nnrc_impish_stmt_free_mcenv_vars s) ψd ->
+        disjoint (nnrc_impish_stmt_bound_mcenv_vars s) ψd ->
+        nnrc_impish_stmt_cross_shadow_free_under s σ ψc ψd.
+    Proof.
+      nnrc_impish_stmt_cases (induction s) Case
+      ; simpl; intros 
+      ; disj_tac
+      ; repeat split
+      ; try solve [
+              tauto
+            | eapply IHs; disj_tac; intuition
+            | eapply IHs1; disj_tac; intuition
+            | eapply IHs2; disj_tac; intuition].
+    Qed.
+
+    Ltac fresh_simpl_rewriter
+      := repeat autorewrite with nnrc_impish_rename in *
+         ; repeat rewrite in_app_iff in *
+         ; repeat match goal with
+                  | [H: In _ (nnrc_impish_stmt_free_env_vars (nnrc_impish_stmt_rename_env _ _ _)) |- _] => apply nnrc_impish_stmt_free_env_vars_rename_env_in in H
+                  | [H: In _ (nnrc_impish_stmt_free_mcenv_vars (nnrc_impish_stmt_rename_mc _ _ _)) |- _] => apply nnrc_impish_stmt_free_mcenv_vars_rename_mcenv_in in H
+                  | [H: In _ (nnrc_impish_stmt_free_mdenv_vars (nnrc_impish_stmt_rename_md _ _ _)) |- _] => apply nnrc_impish_stmt_free_mdenv_vars_rename_mdenv_in in H
+                  | [H: In _ (remove _ _ _) -> False |- _ ] =>
+                    try rewrite <- remove_in_neq in H by congruence
+                  end
+         ; intuition.
+    
+    Lemma nnrc_impish_stmt_cross_shadow_free_alt_rename_env s v v' :
+      ~ In v' (nnrc_impish_stmt_free_mcenv_vars s) ->
+      ~ In v' (nnrc_impish_stmt_bound_mcenv_vars s )->
+      ~ In v' (nnrc_impish_stmt_free_mdenv_vars s) ->
+      ~ In v' (nnrc_impish_stmt_bound_mdenv_vars s) ->
+      nnrc_impish_stmt_cross_shadow_free_alt s ->
+      nnrc_impish_stmt_cross_shadow_free_alt
+        (nnrc_impish_stmt_rename_env s v v').
+    Proof.
+      nnrc_impish_stmt_cases (induction s) Case
+      ; simpl.
+      - Case "NNRCimpishSeq"%string.
+        fresh_simpl_rewriter.
+      - Case "NNRCimpishLet"%string.
+        match_destr.
+        fresh_simpl_rewriter.
+      - Case "NNRCimpishLetMut"%string.
+        repeat split
+        ; do 2 fresh_simpl_rewriter
+        ; try (match_destr_in H4
+               ; fresh_simpl_rewriter).
+        match_destr; fresh_simpl_rewriter.
+      - Case "NNRCimpishLetMutColl"%string.
+        repeat split
+        ; do 2 fresh_simpl_rewriter
+        ; try (match_destr_in H4
+               ; fresh_simpl_rewriter).
+        match_destr; fresh_simpl_rewriter.
+      - Case "NNRCimpishAssign"%string.
+        trivial.
+      - Case "NNRCimpishPush"%string.
+        trivial.
+      - Case "NNRCimpishFor"%string.
+        match_destr.
+        fresh_simpl_rewriter.
+      - Case "NNRCimpishIf"%string.
+        fresh_simpl_rewriter.
+      - Case "NNRCimpishEither"%string.
+        fresh_simpl_rewriter
+        ; try (match_destr_in H2; fresh_simpl_rewriter)
+        ; match_destr; fresh_simpl_rewriter.
+    Qed.
+
+    Lemma nnrc_impish_stmt_cross_shadow_free_alt_rename_mcenv s v v' :
+      ~ In v' (nnrc_impish_stmt_free_env_vars s) ->
+      ~ In v' (nnrc_impish_stmt_bound_env_vars s )->
+      ~ In v' (nnrc_impish_stmt_free_mdenv_vars s) ->
+      ~ In v' (nnrc_impish_stmt_bound_mdenv_vars s) ->
+      nnrc_impish_stmt_cross_shadow_free_alt s ->
+      nnrc_impish_stmt_cross_shadow_free_alt
+        (nnrc_impish_stmt_rename_mc s v v').
+    Proof.
+      nnrc_impish_stmt_cases (induction s) Case
+      ; simpl.
+      - Case "NNRCimpishSeq"%string.
+        fresh_simpl_rewriter.
+      - Case "NNRCimpishLet"%string.
+        do 2 fresh_simpl_rewriter.
+      - Case "NNRCimpishLetMut"%string.
+        repeat split
+        ; do 2 fresh_simpl_rewriter.
+      - Case "NNRCimpishLetMutColl"%string.
+        repeat split
+        ; do 2 fresh_simpl_rewriter
+        ; try (match_destr_in H4
+               ; fresh_simpl_rewriter).
+        match_destr; fresh_simpl_rewriter.
+      - Case "NNRCimpishAssign"%string.
+        trivial.
+      - Case "NNRCimpishPush"%string.
+        trivial.
+      - Case "NNRCimpishFor"%string.
+        do 2 fresh_simpl_rewriter.
+      - Case "NNRCimpishIf"%string.
+        fresh_simpl_rewriter.
+      - Case "NNRCimpishEither"%string.
+        do 2 fresh_simpl_rewriter.
+    Qed.
+
+    Lemma nnrc_impish_stmt_cross_shadow_free_alt_rename_mdenv s v v' :
+      ~ In v' (nnrc_impish_stmt_free_env_vars s) ->
+      ~ In v' (nnrc_impish_stmt_bound_env_vars s )->
+      ~ In v' (nnrc_impish_stmt_free_mcenv_vars s) ->
+      ~ In v' (nnrc_impish_stmt_bound_mcenv_vars s) ->
+      nnrc_impish_stmt_cross_shadow_free_alt s ->
+      nnrc_impish_stmt_cross_shadow_free_alt
+        (nnrc_impish_stmt_rename_md s v v').
+    Proof.
+      nnrc_impish_stmt_cases (induction s) Case
+      ; simpl.
+      - Case "NNRCimpishSeq"%string.
+        fresh_simpl_rewriter.
+      - Case "NNRCimpishLet"%string.
+        do 2 fresh_simpl_rewriter.
+      - Case "NNRCimpishLetMut"%string.
+        repeat split
+        ; do 2 fresh_simpl_rewriter
+        ; try (match_destr_in H4
+               ; fresh_simpl_rewriter).
+        match_destr; fresh_simpl_rewriter.
+      - Case "NNRCimpishLetMutColl"%string.
+        repeat split
+        ; do 2 fresh_simpl_rewriter
+        ; try (match_destr_in H4
+               ; fresh_simpl_rewriter).
+      - Case "NNRCimpishAssign"%string.
+        trivial.
+      - Case "NNRCimpishPush"%string.
+        trivial.
+      - Case "NNRCimpishFor"%string.
+        do 2 fresh_simpl_rewriter.
+      - Case "NNRCimpishIf"%string.
+        fresh_simpl_rewriter.
+      - Case "NNRCimpishEither"%string.
+        do 2 fresh_simpl_rewriter.
+    Qed.
+
+  End cross_shadow_free_alt.
+
+
+  Section uncross.
+
+    Context (sep:string).
+    Fixpoint nnrc_impish_stmt_uncross_shadow_under
+             (s:nnrc_impish_stmt)
+             (σ ψc ψd:list var)
+      : nnrc_impish_stmt
+      := match s with
+         | NNRCimpishSeq s₁ s₂ =>
+           NNRCimpishSeq
+             (nnrc_impish_stmt_uncross_shadow_under s₁ σ ψc ψd)
+             (nnrc_impish_stmt_uncross_shadow_under s₂ σ ψc ψd)
+         | NNRCimpishLet v e s₀ =>
+           let s₀' := nnrc_impish_stmt_uncross_shadow_under s₀ (v::σ) ψc ψd in
+           let problems :=
+               remove equiv_dec v (nnrc_impish_stmt_free_env_vars s₀')
+                      ++ remove equiv_dec v (nnrc_impish_stmt_bound_env_vars s₀')
+                      ++ (nnrc_impish_stmt_free_mcenv_vars s₀')
+                      ++ (nnrc_impish_stmt_bound_mcenv_vars s₀')
+                      ++ (nnrc_impish_stmt_free_mdenv_vars s₀')
+                      ++ (nnrc_impish_stmt_bound_mdenv_vars s₀')
+           in
+           let v' := fresh_var_from sep v problems in
+           NNRCimpishLet v' e (mk_lazy_lift nnrc_impish_stmt_rename_env s₀' v v')
+         | NNRCimpishLetMut v s₁ s₂ =>
+           let s₁' := nnrc_impish_stmt_uncross_shadow_under s₁ σ ψc (v::ψd) in
+           let s₂' := nnrc_impish_stmt_uncross_shadow_under s₂ (v::σ) ψc ψd in
+           let problems := remove equiv_dec v (nnrc_impish_stmt_free_mdenv_vars s₁')
+                                  ++ remove equiv_dec v (nnrc_impish_stmt_bound_mdenv_vars s₁')
+                                  ++ remove equiv_dec v (nnrc_impish_stmt_free_env_vars s₂')
+                                  ++ remove equiv_dec v (nnrc_impish_stmt_bound_env_vars s₂')
+                                  ++ σ
+                                  ++ ψd
+                                  ++ nnrc_impish_stmt_free_env_vars s₁'
+                                  ++ nnrc_impish_stmt_bound_env_vars s₁'
+                                  ++ nnrc_impish_stmt_free_mcenv_vars s₁'
+                                  ++ nnrc_impish_stmt_bound_mcenv_vars s₁'
+                                  ++ nnrc_impish_stmt_free_mcenv_vars s₂'
+                                  ++ nnrc_impish_stmt_bound_mcenv_vars s₂'
+                                  ++ nnrc_impish_stmt_free_mdenv_vars s₂'
+                                  ++ nnrc_impish_stmt_bound_mdenv_vars s₂' in
+           let v' := fresh_var_from sep v problems in
+           NNRCimpishLetMut v'
+                            (mk_lazy_lift nnrc_impish_stmt_rename_md s₁' v v')
+                            (mk_lazy_lift nnrc_impish_stmt_rename_env s₂' v v')
+         | NNRCimpishLetMutColl v s₁ s₂ =>
+           let s₁' := nnrc_impish_stmt_uncross_shadow_under s₁ σ (v::ψc) ψd in
+           let s₂' := nnrc_impish_stmt_uncross_shadow_under s₂ (v::σ) ψc ψd in
+           let problems :=  remove equiv_dec v (nnrc_impish_stmt_free_mcenv_vars s₁')
+                                   ++ remove equiv_dec v (nnrc_impish_stmt_bound_mcenv_vars s₁')
+                                   ++ remove equiv_dec v (nnrc_impish_stmt_free_env_vars s₂')
+                                   ++ remove equiv_dec v (nnrc_impish_stmt_bound_env_vars s₂')
+                                   ++ σ
+                                   ++ ψd
+                                   ++ ψc
+                                   ++ nnrc_impish_stmt_free_env_vars s₁'
+                                   ++ nnrc_impish_stmt_bound_env_vars s₁'
+                                   ++ nnrc_impish_stmt_free_mdenv_vars s₁'
+                                   ++ nnrc_impish_stmt_bound_mdenv_vars s₁'
+                                   ++ nnrc_impish_stmt_free_mcenv_vars s₂'
+                                   ++ nnrc_impish_stmt_bound_mcenv_vars s₂'
+                                   ++ nnrc_impish_stmt_free_mdenv_vars s₂'
+                                   ++ nnrc_impish_stmt_bound_mdenv_vars s₂' in
+           let v' := fresh_var_from sep v problems in
+           NNRCimpishLetMutColl v' 
+                                (mk_lazy_lift nnrc_impish_stmt_rename_mc s₁' v v')
+                                (mk_lazy_lift nnrc_impish_stmt_rename_env s₂' v v')
+         | NNRCimpishAssign v e =>
+           NNRCimpishAssign v e
+         | NNRCimpishPush v e =>
+           NNRCimpishPush v e
+         | NNRCimpishFor v e s₀ =>
+           let s₀' := nnrc_impish_stmt_uncross_shadow_under s₀ (v::σ) ψc ψd in
+           let problems := remove equiv_dec v (nnrc_impish_stmt_free_env_vars s₀')
+                                  ++ remove equiv_dec v (nnrc_impish_stmt_bound_env_vars s₀')
+                                  ++ (nnrc_impish_stmt_free_mcenv_vars s₀')
+                                  ++ (nnrc_impish_stmt_bound_mcenv_vars s₀')
+                                  ++ (nnrc_impish_stmt_free_mdenv_vars s₀')
+                                  ++ (nnrc_impish_stmt_bound_mdenv_vars s₀') in
+           let v' := fresh_var_from sep v problems in
+           NNRCimpishFor v' e (mk_lazy_lift nnrc_impish_stmt_rename_env s₀' v v')
+         | NNRCimpishIf e s₁ s₂ =>
+           NNRCimpishIf
+             e
+             (nnrc_impish_stmt_uncross_shadow_under s₁ σ ψc ψd)
+             (nnrc_impish_stmt_uncross_shadow_under s₂ σ ψc ψd)
+         | NNRCimpishEither e x₁ s₁ x₂ s₂ =>
+           let s₁' := nnrc_impish_stmt_uncross_shadow_under s₁ (x₁::σ) ψc ψd in
+           let problems₁ :=  remove equiv_dec x₁ (nnrc_impish_stmt_free_env_vars s₁')
+                                    ++ remove equiv_dec x₁ (nnrc_impish_stmt_bound_env_vars s₁')
+                                    ++ (nnrc_impish_stmt_free_mcenv_vars s₁')
+                                    ++ (nnrc_impish_stmt_bound_mcenv_vars s₁')
+                                    ++ (nnrc_impish_stmt_free_mdenv_vars s₁')
+                                    ++ (nnrc_impish_stmt_bound_mdenv_vars s₁') in
+           let x₁' := fresh_var_from sep x₁ problems₁ in
+           let s₂' := nnrc_impish_stmt_uncross_shadow_under s₂ (x₂::σ) ψc ψd in
+           let problems₂ := remove equiv_dec x₂ (nnrc_impish_stmt_free_env_vars s₂')
+                                   ++ remove equiv_dec x₂ (nnrc_impish_stmt_bound_env_vars s₂')
+                                   ++ (nnrc_impish_stmt_free_mcenv_vars s₂')
+                                   ++ (nnrc_impish_stmt_bound_mcenv_vars s₂')
+                                   ++ (nnrc_impish_stmt_free_mdenv_vars s₂')
+                                   ++ (nnrc_impish_stmt_bound_mdenv_vars s₂') in
+           let x₂' := fresh_var_from sep x₂ problems₂ in
+           NNRCimpishEither e
+                            x₁'
+                            (mk_lazy_lift nnrc_impish_stmt_rename_env s₁' x₁ x₁')
+                            x₂'
+                            (mk_lazy_lift nnrc_impish_stmt_rename_env s₂' x₂ x₂')
+         end.
+
+    Definition nnrc_impish_uncross_shadow
+               (s:nnrc_impish)
+      : nnrc_impish
+      :=
+        let s' := nnrc_impish_stmt_uncross_shadow_under (fst s) nil nil (snd s::nil) in
+        let problems := nnrc_impish_stmt_free_env_vars s'
+                                                       ++ nnrc_impish_stmt_bound_env_vars s'
+                                                       ++ nnrc_impish_stmt_free_mcenv_vars s'
+                                                       ++ nnrc_impish_stmt_bound_mcenv_vars s' 
+                                                       ++ remove equiv_dec (snd s) (nnrc_impish_stmt_free_mdenv_vars s')
+                                                       ++ remove equiv_dec (snd s) (nnrc_impish_stmt_bound_mdenv_vars s') in
+        let v' := fresh_var_from sep (snd s) problems in
+        (mk_lazy_lift nnrc_impish_stmt_rename_md s' (snd s) v', v').
+
+  End uncross.
+
+  Section correctness.
+
+    Ltac fresh_prover
+      :=
+        repeat rewrite (mk_lazy_lift_under nnrc_impish_stmt_bound_env_vars_rename_env)          
+        ; repeat rewrite (mk_lazy_lift_under nnrc_impish_stmt_free_mcenv_vars_rename_env)
+        ; repeat rewrite (mk_lazy_lift_under nnrc_impish_stmt_bound_mcenv_vars_rename_env)
+        ; repeat rewrite (mk_lazy_lift_under nnrc_impish_stmt_free_mdenv_vars_rename_env)
+        ; repeat rewrite (mk_lazy_lift_under nnrc_impish_stmt_bound_mdenv_vars_rename_env)
+                 
+        ; repeat rewrite (mk_lazy_lift_under nnrc_impish_stmt_free_env_vars_rename_mcenv)
+        ; repeat rewrite (mk_lazy_lift_under nnrc_impish_stmt_bound_env_vars_rename_mcenv)
+        ; repeat rewrite (mk_lazy_lift_under nnrc_impish_stmt_bound_mcenv_vars_rename_mcenv)
+        ; repeat rewrite (mk_lazy_lift_under nnrc_impish_stmt_free_mdenv_vars_rename_mcenv)
+        ; repeat rewrite (mk_lazy_lift_under nnrc_impish_stmt_bound_mdenv_vars_rename_mcenv)
+
+        ; repeat rewrite (mk_lazy_lift_under nnrc_impish_stmt_free_env_vars_rename_mdenv)
+        ; repeat rewrite (mk_lazy_lift_under nnrc_impish_stmt_bound_env_vars_rename_mdenv)
+        ; repeat rewrite (mk_lazy_lift_under nnrc_impish_stmt_free_mcenv_vars_rename_mdenv)
+        ; repeat rewrite (mk_lazy_lift_under nnrc_impish_stmt_bound_mcenv_vars_rename_mdenv)
+        ; repeat rewrite (mk_lazy_lift_under nnrc_impish_stmt_bound_mdenv_vars_rename_mdenv)
+
+        ; try solve [apply fresh_var_from_incl_nin
+                     ; unfold incl; intros; repeat rewrite in_app_iff; intuition].
+    
+    Lemma nnrc_impish_stmt_uncross_shadow_free_alt sep (s:nnrc_impish_stmt)
+          (σ ψc ψd:list var) :
+      nnrc_impish_stmt_cross_shadow_free_alt 
+        (nnrc_impish_stmt_uncross_shadow_under sep s σ ψc ψd).
+    Proof.
+      revert σ ψc ψd
+      ; nnrc_impish_stmt_cases (induction s) Case
+      ; simpl; intros σ ψc ψd; intros.
+      - Case "NNRCimpishSeq"%string.
+        intuition.
+      - Case "NNRCimpishLet"%string.
+        specialize (IHs (v::σ) ψc ψd).
+        fresh_prover.
+        repeat split; try fresh_prover.
+        apply mk_lazy_lift_prop; trivial; intros neq.
+        apply nnrc_impish_stmt_cross_shadow_free_alt_rename_env; trivial
+        ; apply fresh_var_from_incl_nin
+        ; unfold incl; intros; repeat rewrite in_app_iff; tauto.
+      - Case "NNRCimpishLetMut"%string.
+        specialize (IHs1 σ ψc (v::ψd)).
+        specialize (IHs2 (v::σ) ψc ψd).
+        fresh_prover.
+        repeat split; try fresh_prover.
+        + apply mk_lazy_lift_prop; trivial; intros neq.
+          apply nnrc_impish_stmt_cross_shadow_free_alt_rename_mdenv; trivial
+          ; apply fresh_var_from_incl_nin
+          ; unfold incl; intros; repeat rewrite in_app_iff; tauto.
+        + apply mk_lazy_lift_prop; trivial; intros neq.
+          apply nnrc_impish_stmt_cross_shadow_free_alt_rename_env; trivial
+          ; apply fresh_var_from_incl_nin
+          ; unfold incl; intros; repeat rewrite in_app_iff; tauto.
+      - Case "NNRCimpishLetMutColl"%string.
+        specialize (IHs1 σ (v::ψc) ψd).
+        specialize (IHs2 (v::σ) ψc ψd).
+        fresh_prover.
+        repeat split; try fresh_prover.
+        + apply mk_lazy_lift_prop; trivial; intros neq.
+          apply nnrc_impish_stmt_cross_shadow_free_alt_rename_mcenv; trivial
+          ; apply fresh_var_from_incl_nin
+          ; unfold incl; intros; repeat rewrite in_app_iff; tauto.
+        + apply mk_lazy_lift_prop; trivial; intros neq.
+          apply nnrc_impish_stmt_cross_shadow_free_alt_rename_env; trivial
+          ; apply fresh_var_from_incl_nin
+          ; unfold incl; intros; repeat rewrite in_app_iff; tauto.
+      - Case "NNRCimpishAssign"%string.
+        trivial.
+      - Case "NNRCimpishPush"%string.
+        trivial.
+      - Case "NNRCimpishFor"%string.
+        specialize (IHs (v::σ) ψc ψd).
+        fresh_prover.
+        repeat split; try fresh_prover.
+        apply mk_lazy_lift_prop; trivial; intros neq.
+        apply nnrc_impish_stmt_cross_shadow_free_alt_rename_env; trivial
+        ; apply fresh_var_from_incl_nin
+        ; unfold incl; intros; repeat rewrite in_app_iff; tauto.
+      - Case "NNRCimpishIf"%string.
+        intuition.
+      - Case "NNRCimpishEither"%string.
+        specialize (IHs1 (v::σ) ψc ψd).
+        specialize (IHs2 (v0::σ) ψc ψd).
+        fresh_prover.
+        repeat split; try fresh_prover
+        ; apply mk_lazy_lift_prop; trivial; intros neq
+        ; apply nnrc_impish_stmt_cross_shadow_free_alt_rename_env; trivial
+        ; apply fresh_var_from_incl_nin
+        ; unfold incl; intros; repeat rewrite in_app_iff; tauto.
+    Qed.
+
+    Theorem nnrc_impish_uncross_shadow_free sep (s:nnrc_impish) :
+      nnrc_impish_cross_shadow_free (nnrc_impish_uncross_shadow sep s).
+    Proof.
+      destruct s as [s ret]
+      ; unfold nnrc_impish_cross_shadow_free, nnrc_impish_uncross_shadow; simpl.
+      apply nnrc_impish_stmt_cross_shadow_free_under_alt; simpl
+      ; try apply disjoint_nil_r
+      ; try
+          (fresh_prover
+           ; unfold disjoint; simpl; intros ? inn1 inn2; intuition; subst
+           ; apply (fresh_var_from_nincl inn1)
+           ; intros ? inn3
+           ; repeat rewrite in_app_iff in *; tauto).
+      apply mk_lazy_lift_prop; intros.
+      - apply nnrc_impish_stmt_uncross_shadow_free_alt.
+      - apply nnrc_impish_stmt_cross_shadow_free_alt_rename_mdenv; trivial
+        ; try (apply fresh_var_from_incl_nin
+               ; unfold incl; intros; repeat rewrite in_app_iff; tauto).
+        apply nnrc_impish_stmt_uncross_shadow_free_alt.
+    Qed.
+
+    Lemma nnrc_impish_stmt_uncross_shadow_under_eval h c sep (s:nnrc_impish_stmt) σ ψc ψd domσ domψc domψd :
+      nnrc_impish_stmt_eval h c σ ψc ψd (nnrc_impish_stmt_uncross_shadow_under sep s domσ domψc domψd) = nnrc_impish_stmt_eval h c σ ψc ψd s.
+    Proof.
+
+      Ltac prove_freshness 
+        := match goal with
+             [ H: ?v = fresh_var_from _ ?v _ -> False |- _ ] =>
+
+             unfold fresh_var_from in H
+             ; match_destr_in H; try congruence
+             ; apply fresh_var_from_incl_nin
+             ; let a := (fresh "a") in
+               intros a inn; repeat rewrite in_app_iff in *
+               ; destruct (a == v); unfold equiv, complement in *
+               ; [subst; trivial
+                 | eapply remove_in_neq in inn; eauto; try congruence
+                 ]
+           end.
+      
+      revert σ ψc ψd domσ domψc domψd
+      ; nnrc_impish_stmt_cases (induction s) Case
+      ; simpl; intros σ ψc ψd domσ domψc domψd.
+      - Case "NNRCimpishSeq"%string.
+        rewrite IHs1.
+        repeat match_destr.
+      - Case "NNRCimpishLet"%string.
+        match_destr.
+        unfold mk_lazy_lift.
+        dest_eqdec.
+        + rewrite <- e.
+          rewrite IHs; trivial.
+        + rewrite nnrc_impish_stmt_eval_rename_env; try prove_freshness.
+          rewrite IHs; trivial.
+          case_eq (nnrc_impish_stmt_eval h c ((v, Some d) :: σ) ψc ψd s )
+          ; simpl; trivial; intros [[??]?] eqq.
+          destruct p; trivial.
+          destruct p; trivial.            
+      - Case "NNRCimpishLetMut"%string.
+        unfold mk_lazy_lift.
+        dest_eqdec.
+        + rewrite <- e.
+          rewrite IHs1.
+          match_destr.
+          destruct p as [[??]?]
+          ; destruct m0; trivial
+          ; destruct p0; trivial.
+          rewrite IHs2; trivial.
+        + rewrite nnrc_impish_stmt_eval_rename_mdenv; try prove_freshness.
+          rewrite IHs1.
+          unfold var in *.
+          case_eq (nnrc_impish_stmt_eval h c σ ψc ((v, None) :: ψd) s1)
+          ; simpl; trivial; intros [[??]?] eqq.
+          destruct m0; trivial.
+          destruct p0; simpl.
+          rewrite nnrc_impish_stmt_eval_rename_env; try prove_freshness.
+          rewrite IHs2; trivial.
+          unfold var in *.
+          case_eq (nnrc_impish_stmt_eval h c ((v, o) :: p) m m0 s2)
+          ; simpl; trivial; intros [[??]?] eqq2.
+          destruct p0; trivial.
+          destruct p0; trivial.
+      - Case "NNRCimpishLetMutColl"%string.
+        unfold mk_lazy_lift.
+        dest_eqdec.
+        + rewrite <- e.
+          rewrite IHs1.
+          match_destr.
+          destruct p as [[??]?]
+          ; destruct m; trivial
+          ; destruct p0; trivial.
+          rewrite IHs2; trivial.
+        + rewrite nnrc_impish_stmt_eval_rename_mcenv; try prove_freshness.
+          rewrite IHs1.
+          unfold var in *.
+          case_eq (nnrc_impish_stmt_eval h c σ ((v, nil) :: ψc) ψd s1)
+          ; simpl; trivial; intros [[??]?] eqq.
+          destruct m; trivial.
+          destruct p0; simpl.
+          rewrite nnrc_impish_stmt_eval_rename_env; try prove_freshness.
+          rewrite IHs2; trivial.
+          unfold var in *.
+          case_eq (nnrc_impish_stmt_eval h c ((v, Some (dcoll l)) :: p) m m0 s2)
+          ; simpl; trivial; intros [[??]?] eqq2.
+          destruct p0; trivial.
+          destruct p0; trivial.
+      - Case "NNRCimpishAssign"%string.
+        trivial.
+      - Case "NNRCimpishPush"%string.
+        trivial.
+      - Case "NNRCimpishFor"%string.
+        match_destr.
+        unfold mk_lazy_lift.
+        dest_eqdec.
+        + rewrite <- e.
+          clear e.
+          destruct d; trivial.
+          revert σ ψc ψd domσ domψc domψd.
+          induction l
+          ; simpl; intros σ ψc ψd domσ domψc domψd; trivial.
+          rewrite IHs; trivial.
+          match_destr.
+          destruct p as [[??]?].
+          destruct p; trivial.
+          unfold var in *.
+          apply (IHl p0 m m0 domσ domψc domψd).
+        + destruct d; trivial.
+          revert σ ψc ψd domσ domψc domψd c0.
+          induction l
+          ; simpl; intros σ ψc ψd domσ domψc domψd c0; trivial.
+          rewrite nnrc_impish_stmt_eval_rename_env; try prove_freshness.
+          rewrite IHs.
+          case_eq ( nnrc_impish_stmt_eval h c ((v, Some a) :: σ) ψc ψd s); trivial
+          ; intros [[??]?] eqq2.
+          destruct p; trivial.
+          destruct p; trivial.
+          unfold var in *.
+          apply (IHl p0 m m0 domσ domψc domψd); trivial.
+      - Case "NNRCimpishIf"%string.
+        match_destr.
+        destruct d; trivial.
+        destruct b; eauto.
+      - Case "NNRCimpishEither"%string.
+        match_destr.
+        destruct d; trivial.
+        + unfold mk_lazy_lift.
+          dest_eqdec.
+          *  rewrite <- e.
+             rewrite IHs1; trivial.
+          * rewrite nnrc_impish_stmt_eval_rename_env; try prove_freshness.
+            rewrite IHs1; trivial.
+            case_eq (nnrc_impish_stmt_eval h c ((v, Some d) :: σ) ψc ψd s1 )
+            ; simpl; trivial; intros [[??]?] eqq.
+            destruct p; trivial.
+            destruct p; trivial.            
+        + unfold mk_lazy_lift.
+          dest_eqdec.
+          *  rewrite <- e.
+             rewrite IHs2; trivial.
+          * rewrite nnrc_impish_stmt_eval_rename_env; try prove_freshness.
+            rewrite IHs2; trivial.
+            case_eq (nnrc_impish_stmt_eval h c ((v0, Some d) :: σ) ψc ψd s2 )
+            ; simpl; trivial; intros [[??]?] eqq.
+            destruct p; trivial.
+            destruct p; trivial.            
+    Qed.
+
+    Theorem nnrc_impish_uncross_shadow_eval h c sep (s:nnrc_impish) :
+      nnrc_impish_eval h c (nnrc_impish_uncross_shadow sep s) = nnrc_impish_eval h c s.
+    Proof.
+      destruct s as [s ret]
+      ; unfold nnrc_impish_cross_shadow_free, nnrc_impish_uncross_shadow; simpl.
+      unfold mk_lazy_lift.
+      dest_eqdec.
+      + rewrite <- e.
+        rewrite nnrc_impish_stmt_uncross_shadow_under_eval; trivial.
+      + rewrite nnrc_impish_stmt_eval_rename_mdenv
+        ; [| try prove_freshness ; intuition..].
+
+        rewrite nnrc_impish_stmt_uncross_shadow_under_eval; trivial.
+        destruct (nnrc_impish_stmt_eval h c nil nil ((ret, None) :: nil) s); trivial.
+        destruct p as [[??]?].
+        destruct m0; simpl; trivial.
+        destruct p0; trivial.
+    Qed. 
+
+  End correctness.
   
+  Section core.
+    
+    Lemma nnrc_impish_stmt_uncross_shadow_under_preserves_core_f sep (s:nnrc_impish_stmt) (σ ψc ψd:list var) :
+      nnrc_impish_stmtIsCore s ->
+      nnrc_impish_stmtIsCore (nnrc_impish_stmt_uncross_shadow_under sep s σ ψc ψd).
+    Proof.
+      revert σ ψc ψd
+      ; nnrc_impish_stmt_cases (induction s) Case
+      ; simpl; intros σ ψc ψd sf.
+      - Case "NNRCimpishSeq"%string.
+        intuition.
+      - Case "NNRCimpishLet"%string.
+        destruct sf as [sf1 sf2]; split; trivial.
+        apply mk_lazy_lift_prop; [eauto | intros].
+        apply nnrc_impish_stmt_rename_env_core_f.
+        eauto.
+      - Case "NNRCimpishLetMut"%string.
+        destruct sf as [sf1 sf2]; split; trivial.
+        apply mk_lazy_lift_prop; [eauto | intros].
+        + apply nnrc_impish_stmt_rename_md_core; eauto.
+        + apply mk_lazy_lift_prop; [eauto | intros].
+          apply nnrc_impish_stmt_rename_env_core; eauto.
+      - Case "NNRCimpishLetMutColl"%string.
+        destruct sf as [sf1 sf2]; split; trivial.
+        apply mk_lazy_lift_prop; [eauto | intros].
+        + apply nnrc_impish_stmt_rename_mc_core; eauto.
+        + apply mk_lazy_lift_prop; [eauto | intros].
+          apply nnrc_impish_stmt_rename_env_core; eauto.
+      - Case "NNRCimpishAssign"%string.
+        trivial.
+      - Case "NNRCimpishPush"%string.
+        trivial.
+      - Case "NNRCimpishFor"%string.
+        destruct sf as [sf1 sf2]; split; trivial.
+        apply mk_lazy_lift_prop; [eauto | intros].
+        apply nnrc_impish_stmt_rename_env_core.
+        eauto.
+      - Case "NNRCimpishIf"%string.
+        intuition.
+      - Case "NNRCimpishEither"%string.
+        destruct sf as [sf1 sf2]; split; trivial.
+        split
+        ; (apply mk_lazy_lift_prop; [intuition | intros]
+           ; apply nnrc_impish_stmt_rename_env_core
+           ; intuition).
+    Qed.
+
+    Lemma nnrc_impish_stmt_uncross_shadow_under_preserves_core_b sep (s:nnrc_impish_stmt) (σ ψc ψd:list var) :
+      nnrc_impish_stmtIsCore (nnrc_impish_stmt_uncross_shadow_under sep s σ ψc ψd) ->
+      nnrc_impish_stmtIsCore s.
+    Proof.
+      revert σ ψc ψd
+      ; nnrc_impish_stmt_cases (induction s) Case
+      ; simpl; intros σ ψc ψd sf.
+      - Case "NNRCimpishSeq"%string.
+        intuition eauto.
+      - Case "NNRCimpishLet"%string.
+        destruct sf as [sf1 sf2]; split; trivial.
+        apply mk_lazy_lift_prop_inv in sf2.
+        destruct sf2 as [[??]|[sf2 a]]; [eauto|].
+        apply nnrc_impish_stmt_rename_env_core in a; eauto.
+      - Case "NNRCimpishLetMut"%string.
+        destruct sf as [sf1 sf2].
+        split.
+        + apply mk_lazy_lift_prop_inv in sf1.
+          destruct sf1 as [[??]|[sf1 a]]; [eauto|].
+          apply nnrc_impish_stmt_rename_md_core in a; eauto.
+        + apply mk_lazy_lift_prop_inv in sf2.
+          destruct sf2 as [[??]|[sf2 a]]; [eauto|].
+          apply nnrc_impish_stmt_rename_env_core in a; eauto.
+      - Case "NNRCimpishLetMutColl"%string.
+        destruct sf as [sf1 sf2].
+        split.
+        + apply mk_lazy_lift_prop_inv in sf1.
+          destruct sf1 as [[??]|[sf1 a]]; [eauto|].
+          apply nnrc_impish_stmt_rename_mc_core in a; eauto.
+        + apply mk_lazy_lift_prop_inv in sf2.
+          destruct sf2 as [[??]|[sf2 a]]; [eauto|].
+          apply nnrc_impish_stmt_rename_env_core in a; eauto.
+      - Case "NNRCimpishAssign"%string.
+        trivial.
+      - Case "NNRCimpishPush"%string.
+        trivial.
+      - Case "NNRCimpishFor"%string.
+        destruct sf as [sf1 sf2]; split; trivial.
+        apply mk_lazy_lift_prop_inv in sf2.
+        destruct sf2 as [[??]|[sf2 a]]; [eauto|].
+        apply nnrc_impish_stmt_rename_env_core in a.
+        eauto.
+      - Case "NNRCimpishIf"%string.
+        intuition eauto.
+      - Case "NNRCimpishEither"%string.
+        destruct sf as [sf1 [sf2 sf3]]; split; trivial.
+        split.
+        + apply mk_lazy_lift_prop_inv in sf2.
+          destruct sf2 as [[??]|[sf2 a]]; [eauto|].
+          apply nnrc_impish_stmt_rename_env_core in a.
+          eauto.
+        + apply mk_lazy_lift_prop_inv in sf3.
+          destruct sf3 as [[??]|[sf3 a]]; [eauto|].
+          apply nnrc_impish_stmt_rename_env_core in a.
+          eauto.
+    Qed.
+
+    Lemma nnrc_impish_stmt_uncross_shadow_under_preserves_core
+          sep (s:nnrc_impish_stmt) (σ ψc ψd:list var) :
+      nnrc_impish_stmtIsCore (nnrc_impish_stmt_uncross_shadow_under sep s σ ψc ψd) <->
+      nnrc_impish_stmtIsCore s.
+    Proof.
+      split.
+      - apply  nnrc_impish_stmt_uncross_shadow_under_preserves_core_b.
+      - apply  nnrc_impish_stmt_uncross_shadow_under_preserves_core_f.
+    Qed.
+    
+    Theorem nnrc_impish_uncross_shadow_preserves_core sep (s:nnrc_impish) :
+      nnrc_impishIsCore (nnrc_impish_uncross_shadow sep s) <->
+      nnrc_impishIsCore s.
+    Proof.
+      destruct s as [s ret]
+      ; unfold nnrc_impishIsCore, nnrc_impish_cross_shadow_free, nnrc_impish_uncross_shadow; simpl.
+      apply mk_lazy_lift_prop; intros.
+      - apply nnrc_impish_stmt_uncross_shadow_under_preserves_core.
+      - split; intros HH.
+        + apply nnrc_impish_stmt_rename_md_core in HH; eauto.
+          eapply nnrc_impish_stmt_uncross_shadow_under_preserves_core; eauto.
+        + apply nnrc_impish_stmt_rename_md_core; eauto.
+          apply nnrc_impish_stmt_uncross_shadow_under_preserves_core; trivial.
+    Qed.
+
+  End core.
+  Section examples.
+
+    Local Open Scope nnrc_impish.
+    Local Open Scope string.
+
+    Example expr1 : nnrc_impish_stmt
+      := NNRCimpishLet "x"
+                       (NNRCimpishConst (dnat 3))
+                       (NNRCimpishLetMutColl
+                          "x"
+                          (NNRCimpishLetMutColl
+                             "y"
+                             (NNRCimpishLetMutColl
+                                "x"
+                                (NNRCimpishLetMut
+                                   "x"
+                                   (NNRCimpishAssign "x" (NNRCimpishConst (dnat 5)))
+                                   (NNRCimpishPush "x" (NNRCimpishConst (dnat 4))))
+                                (NNRCimpishPush "x" (NNRCimpishConst (dnat 6))))
+                             (NNRCimpishPush "x" (NNRCimpishConst (dnat 7))))
+                          (NNRCimpishAssign "ret" (NNRCimpishConst (dnat 8)))).
+    Eval vm_compute in (nnrc_impish_stmt_uncross_shadow_under "$" expr1 nil nil nil).
+    
+    Example expr2 : nnrc_impish_stmt
+      := NNRCimpishLet "x"
+                       (NNRCimpishConst (dnat 3))
+                       (NNRCimpishLetMutColl
+                          "x"
+                          (NNRCimpishPush "x" (NNRCimpishConst (dnat 8)))
+                          (NNRCimpishAssign "ret" (NNRCimpishConst (dnat 8)))).
+
+    Eval vm_compute in (nnrc_impish_stmt_uncross_shadow_under "$" expr2 nil nil nil).
+
+    Example expr3 : nnrc_impish_stmt
+      := (NNRCimpishLetMut
+            "x"
+            (NNRCimpishPush "x" (NNRCimpishConst (dnat 8)))
+            (NNRCimpishAssign "ret" (NNRCimpishConst (dnat 8)))).
+
+    Eval vm_compute in (nnrc_impish_stmt_uncross_shadow_under "$" expr3 nil nil nil).
+    
+  End examples.
+
 End NNRCimpishCrossShadow.
