coq/NNRCimpish/Lang/NNRCimpishRename.v
@@ -1,0 +1,1278 @@
+(*
+ * Copyright 2015-2016 IBM Corporation
+ *
+ * Licensed under the Apache License, Version 2.0 (the "License");
+ * you may not use this file except in compliance with the License.
+ * You may obtain a copy of the License at
+ *
+ * http://www.apache.org/licenses/LICENSE-2.0
+ *
+ * Unless required by applicable law or agreed to in writing, software
+ * distributed under the License is distributed on an "AS IS" BASIS,
+ * WITHOUT WARRANTIES OR CONDITIONS OF ANY KIND, either express or implied.
+ * See the License for the specific language governing permissions and
+ * limitations under the License.
+ *)
+
+Require Import String.
+Require Import List.
+Require Import Arith.
+Require Import EquivDec.
+Require Import Morphisms.
+Require Import Arith.
+Require Import Max.
+Require Import Bool.
+Require Import Peano_dec.
+Require Import EquivDec.
+Require Import Decidable.
+Require Import Utils.
+Require Import CommonRuntime.
+Require Import NNRCimpish.
+Require Import NNRCimpishVars.
+Require Import NNRCimpishEval.
+
+Section NNRCimpishRename.
+  Context {fruntime:foreign_runtime}. 
+  Context (h:brand_relation_t).
+
+  Section renames.
+    
+    Fixpoint nnrc_impish_stmt_rename_mc
+             (s:nnrc_impish_stmt) (oldvar newvar:var) : nnrc_impish_stmt
+      := match s with
+         | NNRCimpishSeq s₁ s₂ =>
+           NNRCimpishSeq
+             (nnrc_impish_stmt_rename_mc s₁ oldvar newvar)
+             (nnrc_impish_stmt_rename_mc s₂ oldvar newvar)
+         | NNRCimpishLet v e s₀ =>
+           NNRCimpishLet
+             v e
+             (nnrc_impish_stmt_rename_mc s₀ oldvar newvar)         
+         | NNRCimpishLetMut v s₁ s₂ =>
+           NNRCimpishLetMut
+             v
+             (nnrc_impish_stmt_rename_mc s₁ oldvar newvar)         
+             (nnrc_impish_stmt_rename_mc s₂ oldvar newvar)         
+         | NNRCimpishLetMutColl v s₁ s₂ =>
+           NNRCimpishLetMutColl
+             v
+             (if v == oldvar
+              then s₁
+              else nnrc_impish_stmt_rename_mc s₁ oldvar newvar)
+             (nnrc_impish_stmt_rename_mc s₂ oldvar newvar)
+         | NNRCimpishAssign v e =>
+           NNRCimpishAssign v e
+         | NNRCimpishPush v e =>
+           NNRCimpishPush
+             (if v == oldvar then newvar else v)
+             e
+         | NNRCimpishFor v e s₀ =>
+           NNRCimpishFor
+             v e
+             (nnrc_impish_stmt_rename_mc s₀ oldvar newvar)         
+         | NNRCimpishIf e s₁ s₂ =>
+           NNRCimpishIf
+             e
+             (nnrc_impish_stmt_rename_mc s₁ oldvar newvar)
+             (nnrc_impish_stmt_rename_mc s₂ oldvar newvar)         
+         | NNRCimpishEither e x₁ s₁ x₂ s₂ =>
+           NNRCimpishEither
+             e
+             x₁ (nnrc_impish_stmt_rename_mc s₁ oldvar newvar)
+             x₂ (nnrc_impish_stmt_rename_mc s₂ oldvar newvar)         
+         end.
+
+    Fixpoint nnrc_impish_stmt_rename_md
+             (s:nnrc_impish_stmt) (oldvar newvar:var) : nnrc_impish_stmt
+      := match s with
+         | NNRCimpishSeq s₁ s₂ =>
+           NNRCimpishSeq
+             (nnrc_impish_stmt_rename_md s₁ oldvar newvar)
+             (nnrc_impish_stmt_rename_md s₂ oldvar newvar)
+         | NNRCimpishLet v e s₀ =>
+           NNRCimpishLet
+             v e
+             (nnrc_impish_stmt_rename_md s₀ oldvar newvar)         
+         | NNRCimpishLetMut v s₁ s₂ =>
+           NNRCimpishLetMut
+             v
+             (if v == oldvar
+              then s₁
+              else nnrc_impish_stmt_rename_md s₁ oldvar newvar)
+             (nnrc_impish_stmt_rename_md s₂ oldvar newvar)
+         | NNRCimpishLetMutColl v s₁ s₂ =>
+           NNRCimpishLetMutColl
+             v
+             (nnrc_impish_stmt_rename_md s₁ oldvar newvar)         
+             (nnrc_impish_stmt_rename_md s₂ oldvar newvar)
+         | NNRCimpishAssign v e =>
+           NNRCimpishAssign
+             (if v == oldvar then newvar else v)
+             e
+         | NNRCimpishPush v e =>
+           NNRCimpishPush v e
+
+         | NNRCimpishFor v e s₀ =>
+           NNRCimpishFor
+             v e
+             (nnrc_impish_stmt_rename_md s₀ oldvar newvar)         
+         | NNRCimpishIf e s₁ s₂ =>
+           NNRCimpishIf
+             e
+             (nnrc_impish_stmt_rename_md s₁ oldvar newvar)
+             (nnrc_impish_stmt_rename_md s₂ oldvar newvar)         
+         | NNRCimpishEither e x₁ s₁ x₂ s₂ =>
+           NNRCimpishEither
+             e
+             x₁ (nnrc_impish_stmt_rename_md s₁ oldvar newvar)
+             x₂ (nnrc_impish_stmt_rename_md s₂ oldvar newvar)         
+         end.
+
+    Fixpoint nnrc_impish_expr_rename_env
+             (e:nnrc_impish_expr) (oldvar newvar:var) : nnrc_impish_expr
+      := match e with
+         |  NNRCimpishGetConstant v =>
+            NNRCimpishGetConstant v
+         | NNRCimpishVar v =>
+           NNRCimpishVar
+             (if v == oldvar then newvar else v)
+         | NNRCimpishConst d =>
+           NNRCimpishConst d
+         | NNRCimpishBinop b e₁ e₂ =>
+           NNRCimpishBinop
+             b
+             (nnrc_impish_expr_rename_env e₁ oldvar newvar)
+             (nnrc_impish_expr_rename_env e₂ oldvar newvar)
+         | NNRCimpishUnop u e₀ =>
+           NNRCimpishUnop
+             u
+             (nnrc_impish_expr_rename_env e₀ oldvar newvar)
+         | NNRCimpishGroupBy g ls e₀ =>
+           NNRCimpishGroupBy
+             g ls
+             (nnrc_impish_expr_rename_env e₀ oldvar newvar)
+         end.
+
+    Fixpoint nnrc_impish_stmt_rename_env
+             (s:nnrc_impish_stmt) (oldvar newvar:var) : nnrc_impish_stmt
+      := match s with
+         | NNRCimpishSeq s₁ s₂ =>
+           NNRCimpishSeq
+             (nnrc_impish_stmt_rename_env s₁ oldvar newvar)
+             (nnrc_impish_stmt_rename_env s₂ oldvar newvar)
+         | NNRCimpishLet v e s₀ =>
+           NNRCimpishLet
+             v
+             (nnrc_impish_expr_rename_env e oldvar newvar)
+             (if v == oldvar
+              then s₀
+              else nnrc_impish_stmt_rename_env s₀ oldvar newvar)
+         | NNRCimpishLetMut v s₁ s₂ =>
+           NNRCimpishLetMut
+             v
+             (nnrc_impish_stmt_rename_env s₁ oldvar newvar)
+             (if v == oldvar
+              then s₂
+              else nnrc_impish_stmt_rename_env s₂ oldvar newvar)
+         | NNRCimpishLetMutColl v s₁ s₂ =>
+           NNRCimpishLetMutColl
+             v
+             (nnrc_impish_stmt_rename_env s₁ oldvar newvar)         
+             (if v == oldvar
+              then s₂
+              else nnrc_impish_stmt_rename_env s₂ oldvar newvar)
+         | NNRCimpishAssign v e =>
+           NNRCimpishAssign
+             v
+             (nnrc_impish_expr_rename_env e oldvar newvar)
+         | NNRCimpishPush v e =>
+           NNRCimpishPush
+             v
+             (nnrc_impish_expr_rename_env e oldvar newvar)
+         | NNRCimpishFor v e s₀ =>
+           NNRCimpishFor
+             v
+             (nnrc_impish_expr_rename_env e oldvar newvar)
+             (if v == oldvar
+              then s₀
+              else nnrc_impish_stmt_rename_env s₀ oldvar newvar)
+         | NNRCimpishIf e s₁ s₂ =>
+           NNRCimpishIf
+             (nnrc_impish_expr_rename_env e oldvar newvar)
+             (nnrc_impish_stmt_rename_env s₁ oldvar newvar)
+             (nnrc_impish_stmt_rename_env s₂ oldvar newvar)         
+         | NNRCimpishEither e x₁ s₁ x₂ s₂ =>
+           NNRCimpishEither
+             (nnrc_impish_expr_rename_env e oldvar newvar)
+             x₁
+             (if x₁ == oldvar
+              then s₁
+              else nnrc_impish_stmt_rename_env s₁ oldvar newvar)
+             x₂
+             (if x₂ == oldvar
+              then s₂
+              else nnrc_impish_stmt_rename_env s₂ oldvar newvar)
+         end.
+
+  End renames.
+
+  Section rename_vars.
+    
+    Lemma nnrc_impish_expr_free_vars_rename_env e v v' :
+      nnrc_impish_expr_free_vars (nnrc_impish_expr_rename_env e v v')
+      = replace_all (nnrc_impish_expr_free_vars e) v v'.
+    Proof.
+      unfold replace_all.
+      induction e; simpl; trivial.
+      rewrite IHe1, IHe2, map_app; trivial.
+    Qed.
+
+    Lemma nnrc_impish_stmt_free_env_vars_rename_env s v v' :
+      ~ In v' (nnrc_impish_stmt_bound_env_vars s) ->
+      nnrc_impish_stmt_free_env_vars (nnrc_impish_stmt_rename_env s v v')
+      = replace_all (nnrc_impish_stmt_free_env_vars s) v v'.
+    Proof.
+      nnrc_impish_stmt_cases (induction s) Case
+      ; simpl
+      ; intros
+      ; repeat rewrite nnrc_impish_expr_free_vars_rename_env
+      ; repeat rewrite IHs
+      ; repeat rewrite IHs1
+      ; repeat rewrite IHs2
+      ; repeat rewrite IHs3
+      ; repeat rewrite replace_all_app
+      ; repeat rewrite in_app_iff in *
+      ; intuition.
+      - Case "NNRCimpishLet"%string.
+        match_destr.
+        + rewrite e in *; clear e v0.
+          rewrite replace_all_remove_eq.
+          trivial.
+        + rewrite H.
+          rewrite remove_replace_all_comm by congruence.
+          trivial.
+      - Case "NNRCimpishLetMut"%string.
+        match_destr.
+        + rewrite e in *; clear e v0.
+          rewrite replace_all_remove_eq.
+          trivial.
+        + rewrite H3.
+          rewrite remove_replace_all_comm by congruence.
+          trivial.
+      - Case "NNRCimpishLetMutColl"%string.
+        match_destr.
+        + rewrite e in *; clear e v0.
+          rewrite replace_all_remove_eq.
+          trivial.
+        + rewrite H3.
+          rewrite remove_replace_all_comm by congruence.
+          trivial.
+      - Case "NNRCimpishFor"%string.
+        match_destr.
+        + rewrite e in *; clear e v0.
+          rewrite replace_all_remove_eq.
+          trivial.
+        + rewrite H.
+          rewrite remove_replace_all_comm by congruence.
+          trivial.
+      - Case "NNRCimpishEither"%string.
+        repeat match_destr; unfold equiv, complement in *; subst
+        ; repeat rewrite replace_all_remove_eq; trivial.
+        + rewrite H4.
+          rewrite remove_replace_all_comm by congruence.
+          trivial.
+        + rewrite H2.
+          rewrite remove_replace_all_comm by congruence.
+          trivial.
+        + rewrite H2, H4.
+          repeat rewrite remove_replace_all_comm by congruence.
+          trivial.
+    Qed.
+
+    Lemma nnrc_impish_stmt_free_env_vars_rename_env_in s v0 v v' :
+      In v0 (nnrc_impish_stmt_free_env_vars (nnrc_impish_stmt_rename_env s v v')) ->
+      v0 = v' \/ (v0 <> v /\ In v0 (nnrc_impish_stmt_free_env_vars s)).
+    Proof.
+      destruct (v0 == v')
+      ; [left; trivial | ].
+      intros inn; right.
+      nnrc_impish_stmt_cases (induction s) Case
+      ; simpl in *
+      ; repeat rewrite in_app_iff in *
+      ;  repeat rewrite nnrc_impish_expr_free_vars_rename_env in *.
+      - intuition.
+      - Case "NNRCimpishLet"%string.
+        destruct inn as [inn|inn].
+        + apply in_replace_all in inn.
+          intuition.
+        + apply remove_inv in inn.
+          match_destr_in inn; unfold equiv, complement in *; subst
+          ; intuition
+          ; right
+          ; apply remove_in_neq; tauto.
+      - Case "NNRCimpishLetMut"%string.
+        destruct inn as [inn|inn].
+        + intuition.
+        + apply remove_inv in inn.
+          match_destr_in inn; unfold equiv, complement in *; subst
+          ; intuition
+          ; right
+          ; apply remove_in_neq; tauto.
+      - Case "NNRCimpishLetMutColl"%string.
+        destruct inn as [inn|inn].
+        + intuition.
+        + apply remove_inv in inn.
+          match_destr_in inn; unfold equiv, complement in *; subst
+          ; intuition
+          ; right
+          ; apply remove_in_neq; tauto.
+      - Case "NNRCimpishAssign"%string.
+        apply in_replace_all in inn.
+        intuition.
+      - Case "NNRCimpishPush"%string.
+        apply in_replace_all in inn.
+        intuition.
+      - Case "NNRCimpishFor"%string.
+        destruct inn as [inn|inn].
+        + apply in_replace_all in inn.
+          intuition.
+        + apply remove_inv in inn.
+          match_destr_in inn; unfold equiv, complement in *; subst
+          ; intuition
+          ; right
+          ; apply remove_in_neq; tauto.
+      - Case "NNRCimpishIf"%string.
+        destruct inn as [inn|[inn|inn]].
+        + apply in_replace_all in inn.
+          intuition.
+        + intuition.
+        + intuition.
+      - Case "NNRCimpishEither"%string.
+        destruct inn as [inn|[inn|inn]].
+        + apply in_replace_all in inn.
+          intuition.
+        + apply remove_inv in inn.
+          match_destr_in inn; unfold equiv, complement in *; subst
+          ; intuition
+          ; right; left
+          ; apply remove_in_neq; tauto.
+        + apply remove_inv in inn.
+          match_destr_in inn; unfold equiv, complement in *; subst
+          ; intuition
+          ; right; right
+          ; apply remove_in_neq; tauto.
+    Qed.
+
+    Lemma nnrc_impish_stmt_bound_env_vars_rename_env s v v' :
+      nnrc_impish_stmt_bound_env_vars (nnrc_impish_stmt_rename_env s v v')
+      = nnrc_impish_stmt_bound_env_vars s.
+    Proof.
+      induction s; simpl; intuition; try congruence
+      ; repeat (match_destr; try congruence).
+    Qed.
+
+    Lemma nnrc_impish_stmt_free_mcenv_vars_rename_env s v v' :
+      nnrc_impish_stmt_free_mcenv_vars (nnrc_impish_stmt_rename_env s v v')
+      = nnrc_impish_stmt_free_mcenv_vars s.
+    Proof.
+      induction s; simpl; intuition; try congruence
+      ; repeat (match_destr; try congruence).
+    Qed.
+
+    Lemma nnrc_impish_stmt_bound_mcenv_vars_rename_env s v v' :
+      nnrc_impish_stmt_bound_mcenv_vars (nnrc_impish_stmt_rename_env s v v')
+      = nnrc_impish_stmt_bound_mcenv_vars s.
+    Proof.
+      induction s; simpl; intuition; try congruence
+      ; repeat (match_destr; try congruence).
+    Qed.
+
+    Lemma nnrc_impish_stmt_free_mdenv_vars_rename_env s v v' :
+      nnrc_impish_stmt_free_mdenv_vars (nnrc_impish_stmt_rename_env s v v')
+      = nnrc_impish_stmt_free_mdenv_vars s.
+    Proof.
+      induction s; simpl; intuition; try congruence
+      ; repeat (match_destr; try congruence).
+    Qed.
+
+    Lemma nnrc_impish_stmt_bound_mdenv_vars_rename_env s v v' :
+      nnrc_impish_stmt_bound_mdenv_vars (nnrc_impish_stmt_rename_env s v v')
+      = nnrc_impish_stmt_bound_mdenv_vars s.
+    Proof.
+      induction s; simpl; intuition; try congruence
+      ; repeat (match_destr; try congruence).
+    Qed.  
+
+    Lemma nnrc_impish_stmt_free_env_vars_rename_mcenv s v v' :
+      nnrc_impish_stmt_free_env_vars (nnrc_impish_stmt_rename_mc s v v')
+      = nnrc_impish_stmt_free_env_vars s.
+    Proof.
+      induction s; simpl; intuition; try congruence
+      ; repeat (match_destr; try congruence).
+    Qed.
+
+    Lemma nnrc_impish_stmt_bound_env_vars_rename_mcenv s v v' :
+      nnrc_impish_stmt_bound_env_vars (nnrc_impish_stmt_rename_mc s v v')
+      = nnrc_impish_stmt_bound_env_vars s.
+    Proof.
+      induction s; simpl; intuition; try congruence
+      ; repeat (match_destr; try congruence).
+    Qed.
+
+    Lemma nnrc_impish_stmt_free_mcenv_vars_rename_mcenv_in s v0 v v' :
+      In v0 (nnrc_impish_stmt_free_mcenv_vars (nnrc_impish_stmt_rename_mc s v v')) ->
+      v0 = v' \/ (v0 <> v /\ In v0 (nnrc_impish_stmt_free_mcenv_vars s)).
+    Proof.
+      destruct (v0 == v')
+      ; [left; trivial | ].
+      intros inn; right.
+      nnrc_impish_stmt_cases (induction s) Case
+      ; simpl in *
+      ; repeat rewrite in_app_iff in *
+      ; try solve [intuition].
+      - Case "NNRCimpishLetMutColl"%string.
+        destruct inn as [inn|inn].
+        + apply remove_inv in inn.
+          match_destr_in inn; unfold equiv, complement in *; subst
+          ; intuition; left
+          ; apply remove_in_neq; tauto.
+        + intuition.
+      - Case "NNRCimpishPush"%string.
+        match_destr_in inn; intuition; congruence.
+    Qed.
+
+    Lemma nnrc_impish_stmt_bound_mcenv_vars_rename_mcenv s v v' :
+      nnrc_impish_stmt_bound_mcenv_vars (nnrc_impish_stmt_rename_mc s v v')
+      = nnrc_impish_stmt_bound_mcenv_vars s.
+    Proof.
+      induction s; simpl; intuition; try congruence
+      ; repeat (match_destr; try congruence).
+    Qed.
+
+    Lemma nnrc_impish_stmt_free_mdenv_vars_rename_mcenv s v v' :
+      nnrc_impish_stmt_free_mdenv_vars (nnrc_impish_stmt_rename_mc s v v')
+      = nnrc_impish_stmt_free_mdenv_vars s.
+    Proof.
+      induction s; simpl; intuition; try congruence
+      ; repeat (match_destr; try congruence).
+    Qed.
+
+    Lemma nnrc_impish_stmt_bound_mdenv_vars_rename_mcenv s v v' :
+      nnrc_impish_stmt_bound_mdenv_vars (nnrc_impish_stmt_rename_mc s v v')
+      = nnrc_impish_stmt_bound_mdenv_vars s.
+    Proof.
+      induction s; simpl; intuition; try congruence
+      ; repeat (match_destr; try congruence).
+    Qed.
+
+    Lemma nnrc_impish_stmt_free_env_vars_rename_mdenv s v v' :
+      nnrc_impish_stmt_free_env_vars (nnrc_impish_stmt_rename_md s v v')
+      = nnrc_impish_stmt_free_env_vars s.
+    Proof.
+      induction s; simpl; intuition; try congruence
+      ; repeat (match_destr; try congruence).
+    Qed.
+
+    Lemma nnrc_impish_stmt_bound_env_vars_rename_mdenv s v v' :
+      nnrc_impish_stmt_bound_env_vars (nnrc_impish_stmt_rename_md s v v')
+      = nnrc_impish_stmt_bound_env_vars s.
+    Proof.
+      induction s; simpl; intuition; try congruence
+      ; repeat (match_destr; try congruence).
+    Qed.
+
+    Lemma nnrc_impish_stmt_free_mcenv_vars_rename_mdenv s v v' :
+      nnrc_impish_stmt_free_mcenv_vars (nnrc_impish_stmt_rename_md s v v')
+      = nnrc_impish_stmt_free_mcenv_vars s.
+    Proof.
+      induction s; simpl; intuition; try congruence
+      ; repeat (match_destr; try congruence).
+    Qed.
+
+    Lemma nnrc_impish_stmt_bound_mcenv_vars_rename_mdenv s v v' :
+      nnrc_impish_stmt_bound_mcenv_vars (nnrc_impish_stmt_rename_md s v v')
+      = nnrc_impish_stmt_bound_mcenv_vars s.
+    Proof.
+      induction s; simpl; intuition; try congruence
+      ; repeat (match_destr; try congruence).
+    Qed.
+
+    Lemma nnrc_impish_stmt_free_mdenv_vars_rename_mdenv_in s v0 v v' :
+      In v0 (nnrc_impish_stmt_free_mdenv_vars (nnrc_impish_stmt_rename_md s v v')) ->
+      v0 = v' \/ (v0 <> v /\ In v0 (nnrc_impish_stmt_free_mdenv_vars s)).
+    Proof.
+      destruct (v0 == v')
+      ; [left; trivial | ].
+      intros inn; right.
+      nnrc_impish_stmt_cases (induction s) Case
+      ; simpl in *
+      ; repeat rewrite in_app_iff in *
+      ; try solve [intuition].
+      - Case "NNRCimpishLetMut"%string.
+        destruct inn as [inn|inn].
+        + apply remove_inv in inn.
+          match_destr_in inn; unfold equiv, complement in *; subst
+          ; intuition; left
+          ; apply remove_in_neq; tauto.
+        + intuition.
+      - Case "NNRCimpishAssign"%string.
+        match_destr_in inn; intuition; congruence.
+    Qed.
+
+    Lemma nnrc_impish_stmt_bound_mdenv_vars_rename_mdenv s v v' :
+      nnrc_impish_stmt_bound_mdenv_vars (nnrc_impish_stmt_rename_md s v v')
+      = nnrc_impish_stmt_bound_mdenv_vars s.
+    Proof.
+      induction s; simpl; intuition; try congruence
+      ; repeat (match_destr; try congruence).
+    Qed.
+
+    
+  End rename_vars.
+
+  Section rename_eval.
+    
+    Lemma nnrc_impish_expr_eval_rename_env c σ e v v' d:
+      ~ In v' (nnrc_impish_expr_free_vars e) ->
+      nnrc_impish_expr_eval h c ((v', d) :: σ) (nnrc_impish_expr_rename_env e v v')
+      = nnrc_impish_expr_eval h c ((v, d) :: σ) e.
+    Proof.
+      nnrc_impish_expr_cases (induction e) Case; simpl; trivial; intros nin
+      ; try solve [ rewrite IHe by intuition; trivial
+                  |  rewrite IHe1, IHe2 by intuition; trivial
+                  ] .
+      - Case "NNRCimpishVar"%string.
+        intuition.
+        destruct (equiv_dec v0 v)
+        ; repeat (match_destr; try congruence).
+    Qed.
+
+    Lemma nnrc_impish_expr_eval_rename_env_in c l σ e v v' d:
+      ~ In v (domain l) ->
+      ~ In v' (domain l) ->
+      ~ In v' (nnrc_impish_expr_free_vars e) ->
+      nnrc_impish_expr_eval h c (l++(v', d) :: σ) (nnrc_impish_expr_rename_env e v v')
+      = nnrc_impish_expr_eval h c (l++(v, d) :: σ) e.
+    Proof.
+      nnrc_impish_expr_cases (induction e) Case; simpl; trivial
+      ; repeat rewrite in_app_iff; intros
+      ; try solve [ rewrite IHe by intuition; trivial
+                  |  rewrite IHe1, IHe2 by intuition; trivial
+                  ].
+      - Case "NNRCimpishVar"%string.
+        intuition.
+        repeat rewrite lookup_app.
+        destruct (equiv_dec v0 v); unfold equiv, complement in *
+        ; subst.
+        + repeat match_option
+          ; (try apply lookup_in_domain in eqq
+             ; try apply lookup_in_domain in eqq0; try contradiction).
+          simpl.
+          repeat match_destr; congruence.
+        + match_destr; simpl.
+          repeat match_destr; congruence.
+    Qed.
+
+    Ltac disect_tac H stac
+      := 
+        unfold var in *
+        ; cut_to H; unfold domain in *; [ | solve[stac]..]
+        ; unfold lift2P in H
+        ; (repeat match_option_in H; try contradiction).
+
+    Ltac rename_inv_tac1 stac
+      :=    unfold var in *
+            ; repeat rewrite or_assoc
+            ; try match goal with
+                  | [ H: domain (_ ++ _) = domain _ |- _ ] =>
+                    rewrite domain_app in H
+                    ; unfold domain in H
+                    ; symmetry in H; apply map_app_break in H
+                    ; destruct H as [? [?[?[??]]]]; subst; simpl in *
+                  | [ H: map (_ ++ _) = map _ |- _ ] =>
+                    rewrite map_app in H
+                    ; symmetry in H; apply map_app_break in H
+                    ; destruct H as [? [?[?[??]]]]; subst; simpl in *
+                  | [ H: _ :: _ = map _ ?x |- _ ] =>
+                    destruct x; try discriminate; simpl in H; invcs H
+                  | [ H: _ :: _ = domain ?x |- _ ] =>
+                    destruct x; try discriminate; simpl in H; invcs H
+                  | [H: _ * _ * _ |- _ ] => destruct H as [[??]?]; simpl in *
+                  | [H: _ * _ |- _ ] => destruct H as [??]; simpl in *
+                  | [H : nnrc_impish_stmt_eval _ _ ?p1 _ _ _ = Some (?p2,_,_) |- _ ] =>
+                    match p1 with
+                    | p2 => fail 1
+                    | _ => generalize (nnrc_impish_stmt_eval_domain_stack H)
+                           ; intros [?[??]]
+                    end
+                  | [H: ~ (_ \/ _) |- _] => apply not_or in H
+                  | [H: _ /\ _ |- _ ] => destruct H
+                  | [H: ?x = ?x |- _] => clear H
+                  | [ H: forall a b c, _ -> ?x :: ?x1 ++ ?dd :: ?x2 = _ ++ _ :: _ -> _ |- _] =>
+                    specialize (H (x::x1) (snd dd) x2); simpl in H
+                    ; match dd with
+                      | (_,_) => idtac
+                      | _ => destruct dd
+                      end
+                    ; simpl in *
+                    ; cut_to H; [ | eauto 3 | reflexivity]
+                  | [ H: forall a b c, _ -> ?x1 ++ ?dd :: ?x2 = _ ++ _ :: _ -> _ |- _] =>
+                    specialize (H x1 (snd dd) x2)
+                    ; match dd with
+                      | (_,_) => idtac
+                      | _ => destruct dd
+                      end
+                    ; simpl in *
+                    ; cut_to H; [ | eauto 3 | reflexivity]
+                  | [H : ?x ++ _ = ?y ++ _ |- _ ] =>
+                    let HH := fresh in
+                    assert (HH:domain y = domain x) by (unfold domain in *; intuition congruence)
+                    ; apply app_inv_head_domain in H;[clear HH|apply HH]
+                  | [H: _ :: _ = _ :: _ |- _] => invcs H
+                  | [H: ?x = (_,_) |- _ ] =>
+                    match x with
+                    | (_,_) => idtac
+                    | _ => destruct x; simpl in H
+                    end
+                    ; invcs H
+                  | [H: (_,_) = ?x |- _ ] =>
+                    match x with
+                    | (_,_) => fail 1
+                    | _ => destruct x; simpl in H
+                    end
+                    ; invcs H
+                  | [|- _ /\ _ ] => try split; [| tauto]
+                  | [ |- lift2P _ (match ?x with
+                                     _ => _
+                                   end)
+                                (match ?x with
+                                   _ => _
+                                 end) ] => destruct x; try reflexivity
+                  | [H:forall l es ec ed d,
+                        _ -> _ -> _ -> _ -> lift2P _ (nnrc_impish_stmt_eval _ _ _ _ _ ?s) _
+                                                   
+                        |- lift2P _ (nnrc_impish_stmt_eval _ _ (?l ++ (_, ?d) :: ?σ) ?ψc ?ψd ?s)
+                                  _ ] => specialize (H l σ ψc ψd d)
+                                         ; disect_tac H stac
+                                                      
+                  | [H:forall l es ec ed d,
+                        _ -> _ -> _ -> _ -> lift2P _ (nnrc_impish_stmt_eval _ _ _ _ _ ?s) _
+                                                   
+                        |- lift2P _ (match nnrc_impish_stmt_eval _ _ (?l ++ (_, ?d) :: ?σ) ?ψc ?ψd ?s with
+                                     | Some _ => _
+                                     | None => _
+                                     end) _ ] => specialize (H l σ ψc ψd d)
+                                                 ; disect_tac H stac
+                  | [H:forall l es ec ed d,
+                        _ -> _ -> _ -> _ -> lift2P _ (nnrc_impish_stmt_eval _ _ _ _ _ ?s) _
+                                                   
+                        |- lift2P _ (match nnrc_impish_stmt_eval _ _ (?x :: ?l ++ (_, ?d) :: ?σ) ?ψc ?ψd ?s with| Some _ => _
+                                                                                                            | None => _
+                                     end) _ ] => specialize (H (x::l) σ ψc ψd d); simpl in H
+                                                 ; disect_tac H stac
+                  | [H:forall l es ec ed d,
+                        _ -> _ -> _ -> _ -> lift2P _ (nnrc_impish_stmt_eval _ _ _ _ _ ?s) _
+                                                   
+                        |- lift2P _ (nnrc_impish_stmt_eval _ _ ?σ ?ψc (?l ++ (_, ?d) :: ?ψd) ?s)
+                                  _ ] => specialize (H l σ ψc ψd d)
+                                         ; disect_tac H stac
+                                                      
+                  | [H:forall l es ec ed d,
+                        _ -> _ -> _ -> _ -> lift2P _ (nnrc_impish_stmt_eval _ _ _ _ _ ?s) _
+                                                   
+                        |- lift2P _ (match nnrc_impish_stmt_eval _ _ ?σ ?ψc (?l ++ (_, ?d) :: ?ψd) ?s with
+                                     | Some _ => _
+                                     | None => _
+                                     end) _ ] => specialize (H l σ ψc ψd d)
+                                                 ; disect_tac H stac
+                  | [H:forall l es ec ed d,
+                        _ -> _ -> _ -> _ -> lift2P _ (nnrc_impish_stmt_eval _ _ _ _ _ ?s) _
+                                                   
+                        |- lift2P _ (match nnrc_impish_stmt_eval _ _ ?σ ?ψc (?x::?l ++ (_, ?d) :: ?ψd)?s with
+                                     | Some _ => _
+                                     | None => _
+                                     end) _ ] => specialize (H (x::l) σ ψc ψd d); simpl in H
+                                                 ; disect_tac H stac
+                  | [H:forall l es ec ed d,
+                        _ -> _ -> _ -> _ -> lift2P _ (nnrc_impish_stmt_eval _ _ _ _ _ ?s) _
+                                                   
+                        |- lift2P _ (nnrc_impish_stmt_eval _ _ ?σ (?l ++ (_, ?d) :: ?ψc) ?ψd ?s)
+                                  _ ] => specialize (H l σ ψc ψd d)
+                                         ; disect_tac H stac
+                                                      
+                  | [H:forall l es ec ed d,
+                        _ -> _ -> _ -> _ -> lift2P _ (nnrc_impish_stmt_eval _ _ _ _ _ ?s) _
+                                                   
+                        |- lift2P _ (match nnrc_impish_stmt_eval _ _ ?σ (?l ++ (_, ?d) :: ?ψc) ?ψd ?s with
+                                     | Some _ => _
+                                     | None => _
+                                     end) _ ] => specialize (H l σ ψc ψd d)
+                                                 ; disect_tac H stac
+                  | [H:forall l es ec ed d,
+                        _ -> _ -> _ -> _ -> lift2P _ (nnrc_impish_stmt_eval _ _ _ _ _ ?s) _
+                                                   
+                        |- lift2P _ (match nnrc_impish_stmt_eval _ _ ?σ (?x::?l ++ (_, ?d) :: ?ψc) ?ψd ?s  with
+                                     | Some _ => _
+                                     | None => _
+                                     end) _ ] => specialize (H (x::l) σ ψc ψd d); simpl in H
+                                                 ; disect_tac H stac
+
+                  | [H:forall l es ec ed d,
+                        _ -> lift2P _ (nnrc_impish_stmt_eval _ _ _ _ _ ?s) _
+                                    
+                        |- lift2P _ (nnrc_impish_stmt_eval _ _ (?l ++ (_, ?d) :: ?σ) ?ψc ?ψd ?s)
+                                  _ ] => specialize (H l σ ψc ψd d)
+                                         ; disect_tac H stac
+
+                  | [H:forall l es ec ed d,
+                        _ -> lift2P _ (nnrc_impish_stmt_eval _ _ _ _ _ ?s) _
+                                    
+                        |- lift2P _ (match nnrc_impish_stmt_eval _ _ (?l ++ (_, ?d) :: ?σ) ?ψc ?ψd ?s with
+                                     | Some _ => _
+                                     | None => _
+                                     end) _ ] => specialize (H l σ ψc ψd d)
+                                                 ; disect_tac H stac
+                  | [H:forall l es ec ed d,
+                        _ -> lift2P _ (nnrc_impish_stmt_eval _ _ _ _ _ ?s) _
+                                    
+                        |- lift2P _ (match nnrc_impish_stmt_eval _ _ (?x :: ?l ++ (_, ?d) :: ?σ) ?ψc ?ψd ?s with
+                                     | Some _ => _
+                                     | None => _
+                                     end) _ ] => specialize (H (x::l) σ ψc ψd d); simpl in H
+                                                 ; disect_tac H stac
+                  | [H:forall l es ec ed d, 
+                        _ -> lift2P _ (nnrc_impish_stmt_eval _ _ _ _ _ ?s) _
+                                    
+                        |- lift2P _ (nnrc_impish_stmt_eval _ _ ?σ ?ψc (?l ++ (_, ?d) :: ?ψd) ?s)
+                                  _ ] => specialize (H l σ ψc ψd d)
+                                         ; disect_tac H stac
+
+                  | [H:forall l es ec ed d, 
+                        _ -> lift2P _ (nnrc_impish_stmt_eval _ _ _ _ _ ?s) _
+                                    
+                        |- lift2P _ (match nnrc_impish_stmt_eval _ _ ?σ ?ψc (?l ++ (_, ?d) :: ?ψd) ?s with
+                                     | Some _ => _
+                                     | None => _
+                                     end) _ ] => specialize (H l σ ψc ψd d)
+                                                 ; disect_tac H stac
+                  | [H:forall l es ec ed d, 
+                        _ -> lift2P _ (nnrc_impish_stmt_eval _ _ _ _ _ ?s) _
+                                    
+                        |- lift2P _ (match nnrc_impish_stmt_eval _ _ ?σ ?ψc (?x::?l ++ (_, ?d) :: ?ψd) ?s with
+                                     | Some _ => _
+                                     | None => _
+                                     end) _ ] => specialize (H (x::l) σ ψc ψd d); simpl in H
+                                                 ; disect_tac H stac
+                  | [H:forall l es ec ed d, 
+                        _ -> lift2P _ (nnrc_impish_stmt_eval _ _ _ _ _ ?s) _
+                                    
+                        |- lift2P _ (nnrc_impish_stmt_eval _ _ ?σ (?l ++ (_, ?d) :: ?ψc) ?ψd ?s)
+                                  _ ] => specialize (H l σ ψc ψd d)
+                                         ; disect_tac H stac
+
+                  | [H:forall l es ec ed d, 
+                        _ -> lift2P _ (nnrc_impish_stmt_eval _ _ _ _ _ ?s) _
+                                    
+                        |- lift2P _ (match nnrc_impish_stmt_eval _ _ ?σ (?l ++ (_, ?d) :: ?ψc) ?ψd ?s with
+                                     | Some _ => _
+                                     | None => _
+                                     end) _ ] => specialize (H l σ ψc ψd d)
+                                                 ; disect_tac H stac
+                  | [H:forall l es ec ed d, 
+                        _ -> lift2P _ (nnrc_impish_stmt_eval _ _ _ _ _ ?s) _
+                                    
+                        |- lift2P _ (match nnrc_impish_stmt_eval _ _ ?σ (?x::?l ++ (_, ?d) :: ?ψc) ?ψd ?s with
+                                     | Some _ => _
+                                     | None => _
+                                     end) _ ] => specialize (H (x::l) σ ψc ψd d); simpl in H
+                                                 ; disect_tac H stac
+
+                                                              
+                  | [H : ~ In _ (remove equiv_dec _ _) |- _ ] =>
+                    apply not_in_remove_impl_not_in in H; [| congruence]
+                  | [H : In _ (remove equiv_dec _ _) -> False |- _ ] =>
+                    apply not_in_remove_impl_not_in in H; [| congruence]
+                  | [H1: ?x = Some ?y,
+                         H2: ?x = Some ?z |- _ ] =>
+                    rewrite H1 in H2; invcs H2
+                  | [|- ?x = ?y \/ _ ] => destruct (x == y); unfold equiv, complement in *
+                                          ; [left; trivial | right]
+                  end
+            ; try subst; simpl in *; intros
+            ; try congruence
+    .
+    Ltac unused_inv_tac := repeat progress (try rename_inv_tac1 ltac:( unused_inv_tac ; intuition unused_inv_tac); try rewrite nnrc_impish_expr_eval_unused_env by tauto).
+
+    Ltac rename_inv_extra_tac
+      := match goal with
+         | [|- context [nnrc_impish_stmt_eval ?h ?c ((?v1, ?d1) :: ?l ++ (?v2, ?d2) :: ?σ) ?ψc ?ψd ?s ]] =>
+           let HH := fresh in
+           generalize (nnrc_impish_stmt_eval_unused_env h c ((v1,d1)::l) σ ψc ψd s v2 d2); simpl; intros HH; (cut_to HH; [|tauto])
+           ; unfold lift2P in HH
+           ; unfold var in *
+           ; repeat match_option_in HH
+         | [|- context [nnrc_impish_stmt_eval ?h ?c ?σ ?ψc ((?v1, ?d1) :: ?l ++ (?v2, ?d2) :: ?ψd) ?s ]] =>
+           let HH := fresh in
+           generalize (nnrc_impish_stmt_eval_unused_mdenv h c ((v1,d1)::l) σ ψc ψd s v2 d2); simpl; intros HH; (cut_to HH; [|tauto])
+           ; unfold lift2P in HH
+           ; unfold var in *
+           ; repeat match_option_in HH
+         | [|- context [nnrc_impish_stmt_eval ?h ?c ?σ ((?v1, ?d1) :: ?l ++ (?v2, ?d2) :: ?ψc) ?ψd ?s ]] =>
+           let HH := fresh in
+           generalize (nnrc_impish_stmt_eval_unused_mcenv h c ((v1,d1)::l) σ ψc ψd s v2 d2); simpl; intros HH; (cut_to HH; [|tauto])
+           ; unfold lift2P in HH
+           ; unfold var in *
+           ; repeat match_option_in HH
+         end.
+
+    Ltac rename_inv_tac := repeat progress (
+                                    try rename_inv_tac1 ltac:( intuition congruence ; intuition unused_inv_tac)
+                                    ; try rename_inv_extra_tac
+                                    ; repeat rewrite nnrc_impish_expr_eval_rename_env_in by tauto).
+
+
+    Lemma nnrc_impish_stmt_eval_rename_env_in c l σ ψc ψd s (v v':var) d :
+      ~ In v (domain l) ->
+      ~ In v' (domain l) ->
+      ~ In v' (nnrc_impish_stmt_free_env_vars s) ->
+      ~ In v' (nnrc_impish_stmt_bound_env_vars s) ->
+      lift2P  (fun '(σ₁', ψc₁', ψd₁') '(σ₂', ψc₂', ψd₂') =>
+                 (forall l' d σ'',
+                     domain l' = domain l ->
+                     σ₁' = l' ++ (v',d)::σ'' ->
+                     σ₂' = l' ++ (v,d)::σ'')
+                 /\ ψc₁' = ψc₂'
+                 /\ ψd₁' = ψd₂'
+              )
+              (nnrc_impish_stmt_eval h c (l++(v',d)::σ) ψc ψd (nnrc_impish_stmt_rename_env s v v'))
+              (nnrc_impish_stmt_eval h c (l++(v,d)::σ) ψc ψd s).
+    Proof.
+      revert l σ ψc ψd d
+      ; nnrc_impish_stmt_cases (induction s) Case
+      ; simpl; intros l σ ψc ψd d ninl ninl' nine ninb
+      ; repeat rewrite in_app_iff in nine
+      ; repeat rewrite in_app_iff in ninb
+      ; rename_inv_tac
+      ; try solve [dest_eqdec; rename_inv_tac].
+      - Case "NNRCimpishFor"%string.
+        dest_eqdec.
+        + revert σ ψc ψd d.
+          { induction l0; intros σ ψc ψd d; simpl.
+            - rename_inv_tac.
+            - unfold lift2P.
+              generalize (nnrc_impish_stmt_eval_unused_env h c ((v,Some a)::l) σ ψc ψd s v' d); simpl; intros eqs1.
+              cut_to eqs1; [|tauto].
+              generalize (nnrc_impish_stmt_eval_unused_env h c ((v,Some a)::l) σ ψc ψd s v d); simpl; intros eqs2.
+              cut_to eqs2; [|tauto].
+              unfold lift2P in *.
+              unfold var in *.
+              { repeat match_option_in eqs1
+                ; try contradiction
+                ; repeat match_option_in eqs2
+                ; destruct p as [[??]?]
+                ; try contradiction
+                ; destruct p0 as [[??]?]
+                ; try congruence.
+                rename_inv_tac.
+                specialize (IHl0 σ m3 m4 d).
+                repeat match_option_in IHl0
+                ; try contradiction.
+              }
+          }
+        + revert σ ψc ψd d.
+          { induction l0; intros σ ψc ψd d; simpl.
+            - rename_inv_tac. 
+            - unfold lift2P.
+              specialize (IHs ((v0, Some a)::l) σ ψc ψd d).
+              cut_to IHs; simpl; try tauto.
+              unfold lift2P in *; simpl in *.
+              repeat match_option_in IHs
+              ; try contradiction.
+              rename_inv_tac.
+              specialize (IHl0 σ m m0 d).
+              repeat match_option_in IHl0
+              ; try contradiction.
+          }
+    Qed.
+
+    Lemma nnrc_impish_stmt_eval_rename_mdenv_in c l σ ψc ψd s (v v':var) d :
+      ~ In v (domain l) ->
+      ~ In v' (domain l) ->
+      ~ In v' (nnrc_impish_stmt_free_mdenv_vars s) ->
+      ~ In v' (nnrc_impish_stmt_bound_mdenv_vars s) ->
+      lift2P  (fun '(σ₁', ψc₁', ψd₁') '(σ₂', ψc₂', ψd₂') =>
+                 (forall l' d ψd'',
+                     domain l' = domain l ->
+                     ψd₁' = l' ++ (v',d)::ψd'' ->
+                     ψd₂' = l' ++ (v,d)::ψd'')
+                 /\ σ₁' = σ₂'
+                 /\ ψc₁' = ψc₂'
+              )
+              (nnrc_impish_stmt_eval h c σ ψc (l++(v',d)::ψd) (nnrc_impish_stmt_rename_md s v v'))
+              (nnrc_impish_stmt_eval h c σ ψc (l++(v,d)::ψd) s).
+    Proof.
+      revert l σ ψc ψd d
+      ; nnrc_impish_stmt_cases (induction s) Case
+      ; simpl; intros l σ ψc ψd d ninl ninl' nine ninb
+      ; repeat rewrite in_app_iff in nine
+      ; repeat rewrite in_app_iff in ninb
+      ; rename_inv_tac
+      ; try solve [dest_eqdec; rename_inv_tac].
+      - Case "NNRCimpishLetMut"%string.
+        dest_eqdec.
+        + repeat match goal with
+                   [|- context [nnrc_impish_stmt_eval ?h ?c ?σ ?ψc ((?v1, ?d1) :: ?l ++ (?v2, ?d2) :: ?ψd) ?s ]] =>
+                   let HH := fresh in
+                   generalize (nnrc_impish_stmt_eval_unused_mdenv h c ((v1,d1)::l) σ ψc ψd s v2 d2); simpl; intros HH; (cut_to HH; [|tauto])
+                   ; unfold lift2P in HH
+                   ; unfold var in *
+                   ; repeat match_option_in HH
+                 end; try contradiction; try congruence.
+          rewrite eqq0 in eqq2.
+          invcs eqq2.
+          rename_inv_tac; unfold domain in *; try congruence.
+        + rename_inv_tac.
+      - Case "NNRCimpishAssign"%string.
+        repeat rewrite lookup_app; simpl.
+        dest_eqdec.
+        + rewrite (lookup_nin_none string_dec ninl).
+          rewrite (lookup_nin_none string_dec ninl').
+          repeat rewrite update_app_nin by trivial; simpl.
+          destruct (string_dec v v); try congruence.
+          destruct (string_dec v' v'); try congruence.
+          simpl; repeat split; trivial; intros.
+          rename_inv_tac.
+        + destruct (string_dec v0 v'); try congruence.
+          case_eq (lookup string_dec l v0); simpl; [intros ? inn | intros inn].
+          * repeat split; trivial; intros ???? eqq.
+            generalize (lookup_in_domain _ _ inn); intros.
+            rewrite update_app_in in eqq |- * by trivial.
+            apply app_inv_head_domain in eqq
+            ; [| rewrite domain_update_first; trivial].
+            destruct eqq as [eqq1 eqq2].
+            invcs eqq2.
+            congruence.
+          * generalize (lookup_none_nin _ inn); intros.
+            repeat rewrite update_app_nin by trivial.
+            simpl.
+            destruct (string_dec v0 v); try congruence.
+            destruct (string_dec v0 v'); try congruence.
+            match_destr; simpl; trivial.
+            repeat split; trivial; intros ???? eqq.
+            apply app_inv_head_domain in eqq; [| trivial].
+            destruct eqq as [eqq1 eqq2].
+            invcs eqq2.
+            congruence.
+      - Case "NNRCimpishFor"%string.
+        revert l σ ψc ψd d ninl ninl'.
+        induction l0; intros l σ ψc ψd d ninl ninl' ; simpl.
+        + rename_inv_tac. 
+        + unfold lift2P.
+          specialize (IHs l ((v0, Some a)::σ) ψc ψd d).
+          cut_to IHs; simpl; try tauto.
+          unfold lift2P in *; simpl in *.
+          repeat match_option_in IHs
+          ; try contradiction.
+          rename_inv_tac.
+          specialize (IHl0 x1 σ m x2 o0).
+          cut_to IHl0; unfold domain in *; try congruence.
+          repeat match_option_in IHl0
+          ; try contradiction.
+          rename_inv_tac.
+    Qed.
+    
+    Lemma nnrc_impish_stmt_eval_rename_mcenv_in c l σ ψc ψd s (v v':var) d :
+      ~ In v (domain l) ->
+      ~ In v' (domain l) ->
+      ~ In v' (nnrc_impish_stmt_free_mcenv_vars s) ->
+      ~ In v' (nnrc_impish_stmt_bound_mcenv_vars s) ->
+      lift2P  (fun '(σ₁', ψc₁', ψd₁') '(σ₂', ψc₂', ψd₂') =>
+                 (forall l' d ψc'',
+                     domain l' = domain l ->
+                     ψc₁' = l' ++ (v',d)::ψc'' ->
+                     ψc₂' = l' ++ (v,d)::ψc'')
+                 /\ σ₁' = σ₂'
+                 /\ ψd₁' = ψd₂'
+              )
+              (nnrc_impish_stmt_eval h c σ (l++(v',d)::ψc) ψd (nnrc_impish_stmt_rename_mc s v v'))
+              (nnrc_impish_stmt_eval h c σ (l++(v,d)::ψc) ψd s).
+    Proof.
+      revert l σ ψc ψd d
+      ; nnrc_impish_stmt_cases (induction s) Case
+      ; simpl; intros l σ ψc ψd d ninl ninl' nine ninb
+      ; repeat rewrite in_app_iff in nine
+      ; repeat rewrite in_app_iff in ninb
+      ; rename_inv_tac
+      ; try solve [dest_eqdec; rename_inv_tac].
+      - Case "NNRCimpishLetMutColl"%string.
+        dest_eqdec.
+        + repeat match goal with
+                   [|- context [nnrc_impish_stmt_eval ?h ?c ?σ ((?v1, ?d1) :: ?l ++ (?v2, ?d2) :: ?ψc) ?ψd ?s ]] =>
+                   let HH := fresh in
+                   generalize (nnrc_impish_stmt_eval_unused_mcenv h c ((v1,d1)::l) σ ψc ψd s v2 d2); simpl; intros HH; (cut_to HH; [|tauto])
+                   ; unfold lift2P in HH
+                   ; unfold var in *
+                   ; repeat match_option_in HH
+                 end; try contradiction; try congruence.
+          rewrite eqq0 in eqq2.
+          invcs eqq2.
+          rename_inv_tac; unfold domain in *; try congruence.
+        + rename_inv_tac.
+      - Case "NNRCimpishPush"%string.
+        repeat rewrite lookup_app; simpl.
+        dest_eqdec.
+        + rewrite (lookup_nin_none string_dec ninl).
+          rewrite (lookup_nin_none string_dec ninl').
+          destruct (string_dec v v); try congruence.
+          destruct (string_dec v' v'); try congruence.
+          repeat rewrite update_app_nin by trivial; simpl.
+          destruct (string_dec v v); try congruence.
+          destruct (string_dec v' v'); try congruence.
+          simpl; repeat split; trivial; intros.
+          rename_inv_tac.
+        + destruct (string_dec v0 v'); try congruence.
+          case_eq (lookup string_dec l v0); simpl; [intros ? inn | intros inn].
+          * repeat split; trivial; intros ???? eqq.
+            generalize (lookup_in_domain _ _ inn); intros.
+            rewrite update_app_in in eqq |- * by trivial.
+            apply app_inv_head_domain in eqq
+            ; [| rewrite domain_update_first; trivial].
+            destruct eqq as [eqq1 eqq2].
+            invcs eqq2.
+            congruence.
+          * generalize (lookup_none_nin _ inn); intros.
+            simpl.
+            destruct (string_dec v0 v); try congruence.
+            destruct (string_dec v0 v'); try congruence.
+            match_destr; simpl; trivial.
+            repeat rewrite update_app_nin by trivial.
+            simpl.
+            repeat split; trivial; intros ???? eqq.
+            apply app_inv_head_domain in eqq; [| trivial].
+            destruct eqq as [eqq1 eqq2].
+            invcs eqq2.
+            destruct (string_dec v0 v); try congruence.
+            destruct (string_dec v0 v'); try congruence.
+      - Case "NNRCimpishFor"%string.
+        revert l σ ψc ψd d ninl ninl'.
+        induction l0; intros l σ ψc ψd d ninl ninl' ; simpl.
+        + rename_inv_tac. 
+        + unfold lift2P.
+          specialize (IHs l ((v0, Some a)::σ) ψc ψd d).
+          cut_to IHs; simpl; try tauto.
+          unfold lift2P in *; simpl in *.
+          repeat match_option_in IHs
+          ; try contradiction.
+          rename_inv_tac.
+          specialize (IHl0 x1 σ x2 m0 l2).
+          cut_to IHl0; unfold domain in *; try congruence.
+          repeat match_option_in IHl0
+          ; try contradiction.
+          rename_inv_tac.
+    Qed.
+    
+    Lemma nnrc_impish_stmt_eval_rename_env c σ ψc ψd s v v' d:
+      ~ In v' (nnrc_impish_stmt_free_env_vars s) ->
+      ~ In v' (nnrc_impish_stmt_bound_env_vars s) ->
+      nnrc_impish_stmt_eval h c ((v',d)::σ) ψc ψd 
+                            (nnrc_impish_stmt_rename_env s v v') =
+      match nnrc_impish_stmt_eval h c ((v,d)::σ) ψc ψd s with
+      | Some ((_,d)::σ',ψc',ψd') => Some ((v',d)::σ',ψc',ψd')
+      | _ => None
+      end.
+    Proof.
+      intros.
+      generalize (nnrc_impish_stmt_eval_rename_env_in c nil σ ψc ψd s v v' d); simpl; intros HH.
+      cut_to HH; try tauto.
+      unfold lift2P in *.
+      repeat match_option_in HH
+      ; try contradiction.
+      rename_inv_tac; trivial.
+    Qed.
+    
+
+    Lemma nnrc_impish_stmt_eval_rename_mdenv c σ ψc ψd s v v' d:
+      ~ In v' (nnrc_impish_stmt_free_mdenv_vars s) ->
+      ~ In v' (nnrc_impish_stmt_bound_mdenv_vars s) ->
+      nnrc_impish_stmt_eval h c σ ψc ((v',d)::ψd)
+                            (nnrc_impish_stmt_rename_md s v v') =
+      match nnrc_impish_stmt_eval h c σ ψc ((v,d)::ψd) s with
+      | Some (σ',ψc',(_,d)::ψd') => Some (σ',ψc',(v',d)::ψd')
+      | _ => None
+      end.
+    Proof.
+      intros.
+      generalize (nnrc_impish_stmt_eval_rename_mdenv_in c nil σ ψc ψd s v v' d); simpl; intros HH.
+      cut_to HH; try tauto.
+      unfold lift2P in *.
+      repeat match_option_in HH
+      ; try contradiction.
+      rename_inv_tac; trivial.
+      specialize (H1 nil o0 m2).
+      cut_to H1; simpl; try congruence.
+      invcs H1; trivial.
+    Qed.
+
+    Lemma nnrc_impish_stmt_eval_rename_mcenv c σ ψc ψd s v v' d:
+      ~ In v' (nnrc_impish_stmt_free_mcenv_vars s) ->
+      ~ In v' (nnrc_impish_stmt_bound_mcenv_vars s) ->
+      nnrc_impish_stmt_eval h c σ ((v',d)::ψc) ψd
+                            (nnrc_impish_stmt_rename_mc s v v') =
+      match nnrc_impish_stmt_eval h c σ ((v,d)::ψc) ψd s with
+      | Some (σ',(_,d)::ψc',ψd') => Some (σ',(v',d)::ψc',ψd')
+      | _ => None
+      end.
+    Proof.
+      intros.
+      generalize (nnrc_impish_stmt_eval_rename_mcenv_in c nil σ ψc ψd s v v' d); simpl; intros HH.
+      cut_to HH; try tauto.
+      unfold lift2P in *.
+      repeat match_option_in HH
+      ; try contradiction.
+      rename_inv_tac; trivial.
+      specialize (H1 nil l0 m1).
+      cut_to H1; simpl; try congruence.
+      invcs H1; trivial.
+    Qed.
+    
+  End rename_eval.
+
+  Section core.
+
+    Lemma nnrc_impish_expr_rename_env_core e v v' :
+      nnrc_impish_exprIsCore (nnrc_impish_expr_rename_env e v v') <->
+      nnrc_impish_exprIsCore e.
+    Proof.
+      induction e; simpl; intuition.
+    Qed.
+
+    Lemma nnrc_impish_stmt_rename_env_core_f s v v' :
+      nnrc_impish_stmtIsCore s ->
+      nnrc_impish_stmtIsCore (nnrc_impish_stmt_rename_env s v v').
+    Proof.
+      nnrc_impish_stmt_cases (induction s) Case
+      ; simpl; intros isc.
+      - Case "NNRCimpishSeq"%string.
+        intuition.
+      - Case "NNRCimpishLet"%string.
+        destruct isc as [isc1 isc2]; split; trivial.
+        + apply nnrc_impish_expr_rename_env_core; trivial.
+        + match_destr; intuition.
+      - Case "NNRCimpishLetMut"%string.
+        destruct isc as [isc1 isc2]; split; trivial.
+        + intuition.
+        + match_destr; intuition.
+      - Case "NNRCimpishLetMutColl"%string.
+        destruct isc as [isc1 isc2]; split; trivial.
+        + intuition.
+        + match_destr; intuition.
+      - Case "NNRCimpishAssign"%string.
+        apply nnrc_impish_expr_rename_env_core; trivial.
+      - Case "NNRCimpishPush"%string.
+        apply nnrc_impish_expr_rename_env_core; trivial.
+      - Case "NNRCimpishFor"%string.
+        destruct isc as [isc1 isc2]; split; trivial.
+        + apply nnrc_impish_expr_rename_env_core; trivial.
+        + match_destr; intuition.
+      - Case "NNRCimpishIf"%string.
+        destruct isc as [isc1 [isc2 isc3]]; split; trivial.
+        + apply nnrc_impish_expr_rename_env_core; trivial.
+        + split; intuition.
+      - Case "NNRCimpishEither"%string.
+        destruct isc as [isc1 [isc2 isc3]]; split; trivial.
+        + apply nnrc_impish_expr_rename_env_core; trivial.
+        + split; match_destr; intuition.
+    Qed.
+
+    Lemma nnrc_impish_stmt_rename_env_core_b s v v' :
+      nnrc_impish_stmtIsCore (nnrc_impish_stmt_rename_env s v v') ->
+      nnrc_impish_stmtIsCore s.
+    Proof.
+      nnrc_impish_stmt_cases (induction s) Case
+      ; simpl; intros isc.
+      - Case "NNRCimpishSeq"%string.
+        intuition.
+      - Case "NNRCimpishLet"%string.
+        destruct isc as [isc1 isc2].
+        split.
+        + eapply nnrc_impish_expr_rename_env_core; eauto.
+        + match_destr_in isc2; intuition.
+      - Case "NNRCimpishLetMut"%string.
+        destruct isc as [isc1 isc2]; split; trivial.
+        + intuition.
+        + match_destr_in isc2; intuition.
+      - Case "NNRCimpishLetMutColl"%string.
+        destruct isc as [isc1 isc2]; split; trivial.
+        + intuition.
+        + match_destr_in isc2; intuition.
+      - Case "NNRCimpishAssign"%string.
+        eapply nnrc_impish_expr_rename_env_core; eauto.
+      - Case "NNRCimpishPush"%string.
+        eapply nnrc_impish_expr_rename_env_core; eauto.
+      - Case "NNRCimpishFor"%string.
+        destruct isc as [isc1 isc2]; split; trivial.
+        + eapply nnrc_impish_expr_rename_env_core; eauto.
+        + match_destr_in isc2; intuition.
+      - Case "NNRCimpishIf"%string.
+        destruct isc as [isc1 [isc2 isc3]]; split; trivial.
+        + eapply nnrc_impish_expr_rename_env_core; eauto.
+        + split; intuition.
+      - Case "NNRCimpishEither"%string.
+        destruct isc as [isc1 [isc2 isc3]]; split; trivial.
+        + eapply nnrc_impish_expr_rename_env_core; eauto.
+        + split.
+          * match_destr_in isc2; intuition.
+          * match_destr_in isc3; intuition.
+    Qed.
+
+    Lemma nnrc_impish_stmt_rename_env_core s v v' :
+      nnrc_impish_stmtIsCore (nnrc_impish_stmt_rename_env s v v') <->
+      nnrc_impish_stmtIsCore s.
+    Proof.
+      split.
+      - apply nnrc_impish_stmt_rename_env_core_b.
+      - apply nnrc_impish_stmt_rename_env_core_f.
+    Qed.
+
+    Lemma nnrc_impish_stmt_rename_mc_core s v v' :
+      nnrc_impish_stmtIsCore (nnrc_impish_stmt_rename_mc s v v') <->
+      nnrc_impish_stmtIsCore s.
+    Proof.
+      nnrc_impish_stmt_cases (induction s) Case
+      ; simpl; intuition.
+      - match_destr_in H4; intuition.
+      - match_destr; intuition.
+    Qed.
+
+    Lemma nnrc_impish_stmt_rename_md_core s v v' :
+      nnrc_impish_stmtIsCore (nnrc_impish_stmt_rename_md s v v') <->
+      nnrc_impish_stmtIsCore s.
+    Proof.
+      nnrc_impish_stmt_cases (induction s) Case
+      ; simpl; intuition.
+      - match_destr_in H4; intuition.
+      - match_destr; intuition.
+    Qed.
+
+  End core.
+
+End NNRCimpishRename.
+
+Hint Rewrite
+     @nnrc_impish_stmt_bound_env_vars_rename_env 
+     @nnrc_impish_stmt_free_mcenv_vars_rename_env 
+     @nnrc_impish_stmt_bound_mcenv_vars_rename_env 
+     @nnrc_impish_stmt_free_mdenv_vars_rename_env 
+     @nnrc_impish_stmt_bound_mdenv_vars_rename_env 
+     
+     @nnrc_impish_stmt_free_env_vars_rename_mcenv 
+     @nnrc_impish_stmt_bound_env_vars_rename_mcenv 
+     @nnrc_impish_stmt_bound_mcenv_vars_rename_mcenv 
+     @nnrc_impish_stmt_free_mdenv_vars_rename_mcenv 
+     @nnrc_impish_stmt_bound_mdenv_vars_rename_mcenv 
+     
+     @nnrc_impish_stmt_free_env_vars_rename_mdenv 
+     @nnrc_impish_stmt_bound_env_vars_rename_mdenv 
+     @nnrc_impish_stmt_free_mcenv_vars_rename_mdenv 
+     @nnrc_impish_stmt_bound_mcenv_vars_rename_mdenv 
+     @nnrc_impish_stmt_bound_mdenv_vars_rename_mdenv : nnrc_impish_rename.
