coq/Utils/Fresh.v
@@ -40,11 +40,11 @@ Section Fresh.
     
     Fixpoint find_bounded (bound:nat) (init:A)
       := match bound with
-           | O => None
-           | S n =>
-             if f init
-             then Some init
-             else find_bounded n (incr init)
+         | O => None
+         | S n =>
+           if f init
+           then Some init
+           else find_bounded n (incr init)
          end.
 
     Lemma find_bounded_correct bound init y :
@@ -185,7 +185,7 @@ Section Fresh.
     simpl; intuition.
   Qed.
 
-   Lemma fresh_var_fresh3 x1 x2 x3 pre dom :
+  Lemma fresh_var_fresh3 x1 x2 x3 pre dom :
     x3 <> fresh_var pre (x1::x2::x3::dom).
   Proof.
     intro inn.
@@ -239,8 +239,8 @@ Section Fresh.
   (* given a variable, gets the "base": the part before the last seperator *)
   Definition get_var_base (sep:string) (var:string)
     := match index 0 (string_reverse sep) (string_reverse var) with
-         | Some n => substring 0 (String.length var - (S n)) var
-         | None => var
+       | Some n => substring 0 (String.length var - (S n)) var
+       | None => var
        end.
 
   Lemma get_var_base_pre sep var :
@@ -266,50 +266,74 @@ Section Fresh.
   Qed.
 
   Lemma find_fresh_inj_f_equivlist x y :
-      equivlist x y ->
-      find_fresh_inj_f nat_to_string16 nat_to_string16_inj x =
-      find_fresh_inj_f nat_to_string16 nat_to_string16_inj y.
-    Proof.
-      intros.
-      unfold find_fresh_inj_f; simpl.
-      repeat (match goal with
-      | [|- context[ proj1_sig ?x ]] => destruct x
-      end; simpl).
-      apply some_lift in e.
-      destruct e as [? e ?]; subst.
-      apply some_lift in e0.
-      destruct e0 as [? e0 ?]; subst.
-      f_equal.
-      rewrite find_bounded_S_seq in e, e0.
-      rewrite (find_ext
-                 (fun x0 : nat => if in_dec equiv_dec (nat_to_string16 x0) x then false else true)
-                 (fun x0 : nat => if in_dec equiv_dec (nat_to_string16 x0) y then false else true)) in e.
-      - eapply find_seq_same; eauto.
-      - intros.
-        do 2 match_destr.
-        + rewrite H in i; congruence.
-        + rewrite <- H in i; congruence.
-    Qed.
-                     
-    Global Instance find_fresh_string_equivlist : Proper (equivlist ==> eq) find_fresh_string.
-    Proof.
-      intros ???.
-      unfold find_fresh_string.
-      apply find_fresh_inj_f_equivlist; trivial.      
-    Qed.
+    equivlist x y ->
+    find_fresh_inj_f nat_to_string16 nat_to_string16_inj x =
+    find_fresh_inj_f nat_to_string16 nat_to_string16_inj y.
+  Proof.
+    intros.
+    unfold find_fresh_inj_f; simpl.
+    repeat (match goal with
+            | [|- context[ proj1_sig ?x ]] => destruct x
+            end; simpl).
+    apply some_lift in e.
+    destruct e as [? e ?]; subst.
+    apply some_lift in e0.
+    destruct e0 as [? e0 ?]; subst.
+    f_equal.
+    rewrite find_bounded_S_seq in e, e0.
+    rewrite (find_ext
+               (fun x0 : nat => if in_dec equiv_dec (nat_to_string16 x0) x then false else true)
+               (fun x0 : nat => if in_dec equiv_dec (nat_to_string16 x0) y then false else true)) in e.
+    - eapply find_seq_same; eauto.
+    - intros.
+      do 2 match_destr.
+      + rewrite H in i; congruence.
+      + rewrite <- H in i; congruence.
+  Qed.
+  
+  Global Instance find_fresh_string_equivlist : Proper (equivlist ==> eq) find_fresh_string.
+  Proof.
+    intros ???.
+    unfold find_fresh_string.
+    apply find_fresh_inj_f_equivlist; trivial.      
+  Qed.
   (*
 Eval vm_compute in 
       fresh_var_from "$"%string "cat_var$5"%string ("cat_var$0"::"i"::"cat_var$5"::"tmp1"::"tmp2"::"cat_var1"::nil)%string.
-*)
+   *)
 
-    Global Instance fresh_var_equivlist : Proper (eq ==> equivlist ==> eq) fresh_var.
-    Proof.
-      intros ??????; subst.
-      unfold fresh_var.
-      rewrite H0.
-      reflexivity.
-    Qed.
-    
+  Global Instance fresh_var_equivlist : Proper (eq ==> equivlist ==> eq) fresh_var.
+  Proof.
+    intros ??????; subst.
+    unfold fresh_var.
+    rewrite H0.
+    reflexivity.
+  Qed.
+
+  Lemma fresh_var_from_id sep v l :
+    ~ In v l ->
+    fresh_var_from sep v l = v.
+  Proof.
+    unfold fresh_var_from.
+    match_destr; tauto.
+  Qed.
+
+  Lemma fresh_var_from_nincl {sep v l l2} :
+    In (fresh_var_from sep v l) l2 -> ~ incl l2 l.
+  Proof.
+    intros inn1 incl.
+    apply (fresh_var_from_fresh sep v l).
+    apply incl; trivial.
+  Qed.
+
+  Lemma fresh_var_from_incl_nin sep v l1 l2 :
+    incl l2 l1 ->
+    ~ In (fresh_var_from sep v l1) l2.
+  Proof.
+    intros incl1 inn.
+    apply (fresh_var_from_nincl inn); trivial.
+  Qed.
+
 End Fresh.
 
 Ltac prove_fresh_nin
